port everything except theorems

HL/Equiv.lean
@@ -19,33 +19,22 @@ file := some "Equiv"
 open scoped HasEval MyGetElem Com
 ```
 
-:::dev "Sati (satiscugcat)"
-  At this point, the Rocq file provides instructions about using a new directory,
-  making sure the project is set up properly, and also instructions about how to
-  deal with the exercises. I am assuming these things are being moved to Intro.lean?
-  I am excluding them for now.
-:::
+# Behavioral Equivalence
 
-```lean
-open scoped HasEval MyGetElem
-```
-
-# Behavioral Equivaleence
 ::::full
+In {ref "Slang"}[an earlier chapter], we investigated the correctness of a very
+simple program transformation: the `optimize0plus` function.  The
+programming language we were considering was the first version of
+the language of arithmetic expressions - with no variables - so
+in that setting it was very easy to define what it means for a
+program transformation to be correct: it should always yield a
+program that evaluates to the same number as the original.
 
-  In an earlier chapter, we investigated the correctness of a very
-  simple program transformation: the `optimize0plus` function.  The
-  programming language we were considering was the first version of
-  the language of arithmetic expressions -- with no variables -- so
-  in that setting it was very easy to define what it means for a
-  program transformation to be correct: it should always yield a
-  program that evaluates to the same number as the original.
-
-  To talk about the correctness of program transformations for the
-  full Imp language -- in particular, assignment -- we need to
-  consider the role of mutable state and develop a more
-  sophisticated notion of correctness, which we'll call _behavioral
-  equivalence_.
+To talk about the correctness of program transformations for the
+full Imp language - in particular, assignment - we need to
+consider the role of mutable state and develop a more
+sophisticated notion of correctness, which we'll call _behavioral
+equivalence_.
 ::::
 
 ::::full
@@ -58,8 +47,8 @@ For example:
 ## Definitions
 
 ::::full
-For `aexp`s and `bexp`s with variables, the definition we want is
-clear: Two `aexp`s or `bexp`s are "behaviorally equivalent" if
+For `Aexp`s and `Bexp`s with variables, the definition we want is
+clear: Two `Aexp`s or `Bexp`s are "behaviorally equivalent" if
 they evaluate to the same result in every state.
 ::::
 
@@ -68,17 +57,36 @@ def Aexp.Equiv (a₁ a₂ : Aexp) : Prop :=
   ∀ (st : State),
     a₁.eval st = a₂.eval st
 
-theorem Aexp.equiv_def {a₁ a₂ : Aexp} :
-    a₁.Equiv a₂ ↔ ∀ (st : State), a₁.eval st = a₂.eval st := by rfl
-```
-
-```lean
 def Bexp.Equiv (b₁ b₂ : Bexp) : Prop :=
   ∀ (st : State),
     b₁.eval st = b₂.eval st
+```
 
+We'll also define a notation for `Equiv`:
+
+```lean
+class Equiv (α : Type) where
+  equiv : α → α → Prop
+
+infix:70 " ≃ " => Equiv.equiv -- you can type `≃` as \equiv
+
+instance : Equiv Aexp where
+  equiv := Aexp.Equiv
+
+instance : Equiv Bexp where
+  equiv := Bexp.Equiv
+
+@[simp]
+theorem Aexp.equiv_notation {a₁ a₂ : Aexp} : a₁.Equiv a₂ ↔ a₁ ≃ a₂ := by rfl
+@[simp]
+theorem Aexp.equiv_def {a₁ a₂ : Aexp} :
+    a₁ ≃ a₂ ↔ ∀ (st : State), a₁.eval st = a₂.eval st := by rfl
+
+@[simp]
+theorem Bexp.equiv_notation {b₁ b₂ : Bexp} : b₁.Equiv b₂ ↔ b₁ ≃ b₂ := by rfl
+@[simp]
 theorem Bexp.equiv_def {b₁ b₂ : Bexp} :
-    b₁.Equiv b₂ ↔ ∀ (st : State), b₁.eval st = b₂.eval st := by rfl
+    b₁ ≃ b₂ ↔ ∀ (st : State), b₁.eval st = b₂.eval st := by rfl
 ```
 
 ::::full
@@ -87,45 +95,41 @@ and boolean expressions.
 ::::
 
 ```lean
-example : Aexp.Equiv
-    (aexp { X - X })
-    (aexp { 0 }) := by
-  rw [Aexp.equiv_def]
-  intro st
-  simp
+example : aexp { X - X } ≃ aexp { 0 } := by simp
 ```
 
 
 ```lean
-example : Bexp.Equiv
-    (bexp { X - X = 0 })
-    (bexp { true }) := by
-  rw [Bexp.equiv_def]
-  intro st
-  simp
+example : bexp { X - X = 0 } ≃ bexp { true } := by simp
 ```
 
 ::::full
-  For commands, the situation is a little more subtle.  We
-  can't simply say "two commands are behaviorally equivalent if they
-  evaluate to the same ending state whenever they are started in the
-  same initial state," because some commands, when run in some
-  starting states, don't terminate in any final state at all!
+For commands, the situation is a little more subtle.  We
+can't simply say "two commands are behaviorally equivalent if they
+evaluate to the same ending state whenever they are started in the
+same initial state," because some commands, when run in some
+starting states, don't terminate in any final state at all!
 
-  What we need instead is this: two commands are behaviorally
-  equivalent if, for any given starting state, they either (1) both
-  diverge or else (2) both terminate in the same final state.  A
-  compact way to express this is "if the first one terminates in a
-  particular state then so does the second, and vice versa."
+What we need instead is this: two commands are behaviorally
+equivalent if, for any given starting state, they either (1) both
+diverge or else (2) both terminate in the same final state.  A
+compact way to express this is "if the first one terminates in a
+particular state then so does the second, and vice versa."
 ::::
 
 ```lean
 def Com.Equiv (c₁ c₂ : Com) : Prop :=
     ∀ {st st' : State},
-      (st =[ ~c₁ ]=> st') ↔ (st =[ ~c₂ ]=> st')
+      (st =[ c₁ ]=> st') ↔ (st =[ c₂ ]=> st')
 
-theorem Com.equiv_def {c₁ c₂ : Com} : c₁.Equiv c₂ ↔
-    ∀ {st st' : State}, (st =[ ~c₁ ]=> st') ↔ (st =[ ~c₂ ]=> st') := by rfl
+instance : Equiv Com where
+  equiv := Com.Equiv
+
+@[simp]
+theorem Com.equiv_notation {c₁ c₂ : Com} : c₁.Equiv c₂ ↔ c₁ ≃ c₂ := by rfl
+@[simp]
+theorem Com.equiv_def {c₁ c₂ : Com} : c₁ ≃ c₂ ↔
+    ∀ {st st' : State}, (st =[ c₁ ]=> st') ↔ (st =[ c₂ ]=> st') := by rfl
 ```
 
 ## Simple Examples
@@ -136,11 +140,11 @@ namespace Com
 
 ::::full
   For examples of command equivalence, let's start by looking at
-  a trivial equivalence involving `skip`.
+  a trivial equivalence involving {name}`skip`.
 ::::
 
 ```lean
-theorem skip_left {c : Com} : (imp { skip; ~c }).Equiv c := by
+theorem skip_left {c : Com} : imp { skip; c } ≃ c := by
   workinclass!
     rw [equiv_def]
     intro st st''
@@ -155,11 +159,11 @@ theorem skip_left {c : Com} : (imp { skip; ~c }).Equiv c := by
 ```
 
 :::::exercise (rating := 2) (name:= "skip_right")
-Prove that adding a `skip` _after_ a command also results in an
+Prove that adding a {name}`skip` _after_ a command also results in an
 equivalent program.
 
 ```lean
-theorem skip_right {c : Com} : (imp { ~c; skip }).Equiv c := by
+theorem skip_right {c : Com} : imp { c; skip } ≃ c := by
   solution!
     rw [equiv_def]
     intro st st''
@@ -180,7 +184,7 @@ commands.
 ::::
 
 ```lean
-theorem if_true_simple {c₁ c₂ : Com} : (imp {if (true) {~c₁} else {~c₂}}).Equiv c₁ := by
+theorem if_true_simple {c₁ c₂ : Com} : imp {if (true) {c₁} else {c₂}} ≃ c₁ := by
   rw [equiv_def]
   intro st st'
   constructor
@@ -195,52 +199,47 @@ theorem if_true_simple {c₁ c₂ : Com} : (imp {if (true) {~c₁} else {~c₂}}
 
 ::::full
 Of course, no programmer would write a conditional whose condition
-is literally `true`.  (At least, no human programmer -- compilers
+is literally `true`.  (At least, no human programmer - compilers
 and macro preprocessors do this sort of thing internally all the
 time!) But they might write one whose condition is _equivalent_ to
 true:
 ::::
-:::dev "Sati (satiscugcat)"
-The to\_verso script seems to use `\[\]` blocks, but these seem to
-cause problems with the tilde. Currently skipping them and just using
-backticks.
-:::
+
 ::::full
-_Theorem_: If `b` is equivalent to `true`, then `if (~b) {~c₁}
-else {~c₂}` is equivalent to `c₁`.
+_Theorem_: If `b` is equivalent to `true`, then `if (b) {c₁} else {c₂}` is equivalent to `c₁`.
 _Proof_:
- - (`->`) We must show, for all `st` and `st'`, that if
-   `st =[ imp {if (~b) {~c₁} else {~c₂}} ]=> st'` then
+ - (`→`) We must show, for all `st` and `st'`, that if
+   `st =[ imp {if (b) {c₁} else {c₂}} ]=> st'` then
    `st =[ c₁ ]=> st'`.
 
    Proceed by cases on the rules that could possibly have been
-   used to show `st =[ imp {if (~b) {~c₁} else {~c₂}} ]=> st'`,
-   namely `Com.EvalR.ifTrue` and `Com.EvalR.ifFalse`.
+   used to show `st =[ imp {if (b) {c₁} else {c₂}} ]=> st'`,
+   namely {name}`Com.EvalR.ifTrue` and {name}`Com.EvalR.ifFalse`.
 
    - Suppose the final rule in the derivation of
-     `st =[ imp {if (~b) {~c₁} else {~c₂}} ]=> st'` was `Com.EvalR.ifTrue`.
-     We then have, by the premises of `Com.EvalR.ifTrue`, that
+     `st =[ imp {if (b) {c₁} else {c₂}} ]=> st'` was {name}`Com.EvalR.ifTrue`.
+     We then have, by the premises of {name}`Com.EvalR.ifTrue`, that
      `st =[ c₁ ]=> st'`. This is exactly what we set out to prove.
 
    - On the other hand, suppose the final rule in the derivation
-     of `st =[ imp {if (~b) {~c₁} else {~c₂}} ]=> st'` was `Com.EvalR.ifFalse`.
+     of `st =[ imp {if (b) {c₁} else {c₂}} ]=> st'` was `Com.EvalR.ifFalse`.
      We then know that `b.eval st = false` and `st =[ c₂ ]=> st'`.
 
      Recall that `b` is equivalent to `true`, i.e., forall `st`,
-     `b.eval st = (bexp {true}).eval st`.  In particular, this means
-     that `b.eval st = true`, since `(bexp {true}).eval st = true`.  But
-     this is a contradiction, since `Com.EvalR.ifFalse` requires that
+     `b.eval st = (Bexp {true}).eval st`.  In particular, this means
+     that `b.eval st = true`, since `(Bexp {true}).eval st = true`.  But
+     this is a contradiction, since {name}`Com.EvalR.ifFalse` requires that
      `b.eval st = false`.  Thus, the final rule could not have
-     been `Com.EvalR.ifFalse`.
+     been {name}`Com.EvalR.ifFalse`.
 
  - (`<-`) We must show, for all `st` and `st'`, that if
    `st =[ c₁ ]=> st'` then
-   `st =[ imp {if (~b) {~c₁} else {~c₂}} ]=> st'`.
+   `st =[ imp {if (b) {c₁} else {c₂}} ]=> st'`.
 
    Since `b` is equivalent to `true`, we know that `b.eval st` =
-   `(bexp {true}).eval st = true` = `true`.  Together with the assumption that
-   `st =[ c₁ ]=> st'`, we can apply `Com.EvalR.ifTrue` to derive
-   `st =[ imp {if (~b) {~c₁} else {~c₂}} ]=> st'`.
+   `(Bexp {true}).eval st = true` = `true`.  Together with the assumption that
+   `st =[ c₁ ]=> st'`, we can apply {name}`Com.EvalR.ifTrue` to derive
+   `st =[ imp {if (b) {c₁} else {c₂}} ]=> st'`.
 ::::
 
 ::::full
@@ -248,45 +247,31 @@ Here is the formal version of this proof:
 ::::
 
 ```lean
-theorem if_true {b : Bexp} {c₁ c₂ : Com} (hb : b.Equiv (bexp {true})) :
-    (imp {if (~b) {~c₁} else {~c₂}}).Equiv c₁ := by
+theorem if_true {b : Bexp} {c₁ c₂ : Com} (hb : b ≃ bexp {true}) :
+    imp {if (b) {c₁} else {c₂}} ≃ c₁ := by
   rw [equiv_def]
-  rw [Bexp.equiv_def] at hb
   intro st st'
   constructor
   · intro h
-    inversion h with
-    | ifTrue hb' hc =>
-      exact hc
-    | ifFalse hb' hc =>
-      rw [hb] at hb'
-      simp at hb'
+    inversion h <;> simp_all
   · intro h
     apply EvalR.ifTrue _ h
-    rw [hb]
-    simp
+    simp_all
 ```
 
 :::::exercise (rating := 2) (name := "if_false_equiv")
 ```lean
-theorem if_false {b : Bexp} {c₁ c₂ : Com} (hb : b.Equiv (bexp {false})) :
-    (imp {if (~b) {~c₁} else {~c₂}}).Equiv c₂ := by
+theorem if_false {b : Bexp} {c₁ c₂ : Com} (hb : b ≃ bexp {false}) :
+    imp {if (b) {c₁} else {c₂}} ≃ c₂ := by
   solution!
     rw [equiv_def]
-    rw [Bexp.equiv_def] at hb
     intro st st'
     constructor
     · intro h
-      inversion h with
-      | ifTrue hb' hc =>
-        rw [hb] at hb'
-        simp at hb'
-      | ifFalse hb' hc =>
-        exact hc
+      inversion h <;> simp_all
     · intro h
       apply EvalR.ifFalse _ h
-      rw [hb]
-      simp
+      simp_all
 ```
 :::::
 
@@ -297,8 +282,8 @@ condition.
 
 ```lean
 theorem swap_if_branches {b : Bexp} {c₁ c₂ : Com} :
-    (imp {if (~b) {~c₁} else {~c₂}}).Equiv
-    (imp {if (¬ ~b) {~c₂} else {~c₁}}) := by
+    imp {if (b) {c₁} else {c₂}} ≃
+    imp {if (¬ b) {c₂} else {c₁}} := by
   solution!
     rw [equiv_def]
     intro st st'
@@ -324,9 +309,9 @@ theorem swap_if_branches {b : Bexp} {c₁ c₂ : Com} :
 
 ::::full
 For `while` loops, we can give a similar pair of theorems.  A loop
-whose guard is equivalent to `false` is equivalent to `skip`,
-while a loop whose guard is equivalent to `true` is equivalent to
-`while (true) {skip;} end` (or any other non-terminating program).
+whose guard is equivalent to {name}`false` is equivalent to {name}`skip`,
+while a loop whose guard is equivalent to {name}`true` is equivalent to
+`while (true) {skip} end` (or any other non-terminating program).
 ::::
 
 ::::full
@@ -334,22 +319,20 @@ The first of these facts is easy.
 ::::
 
 ```lean
-theorem while_false_equiv {b : Bexp} {c : Com} (hb : b.Equiv (bexp {false})) :
-    (imp {while (~b) {~c}}).Equiv
-    (imp {skip}) := by
+theorem while_false_equiv {b : Bexp} {c : Com} (hb : b ≃ bexp {false}) :
+    imp {while (b) {c}} ≃ imp {skip} := by
   rw [equiv_def]
-  rw [Bexp.equiv_def] at hb
   intro st st''
   constructor
   · intro h
     inversion h with
     | whileFalse => exact EvalR.skip
     | whileTrue st' hb' hc hloop =>
-      simp [hb] at hb'
+      simp_all
   · intro h
     inversion h
     apply EvalR.whileFalse
-    simp [hb]
+    simp_all
 ```
 
 :::::exercise (rating := 2) (name := "while_false_informal") (level:= Advanced) (manual:= true)
@@ -358,65 +341,64 @@ Write an informal proof of `while_false_equiv`.
 
 ::::full
 To prove the second fact, we need an auxiliary lemma stating that
-`while` loops whose guards are equivalent to `true` never
+`while` loops whose guards are equivalent to {name}`true` never
 terminate.
 ::::
 
 ::::full
-_Lemma_: If `b` is equivalent to `true`, then it cannot be
-the case that `st =[ while (~b) {~c} ]=> st'`.
+_Lemma_: If `b` is equivalent to {name}`true`, then it cannot be
+the case that `st =[ while (b) {c} ]=> st'`.
 
-_Proof_: Suppose that `st =[ while (~b) {~c} ]=> st'`.  We show,
-by induction on a derivation of `st =[ while (~b) {~c} ]=> st'`,
+_Proof_: Suppose that `st =[ while (b) {c} ]=> st'`.  We show,
+by induction on a derivation of `st =[ while (b) {c} ]=> st'`,
 that this assumption leads to a contradiction. The only two cases
-to consider are `Com.EvalR.whileFalse` and `Com.EvalR.whileTrue`; the others
+to consider are {name}`Com.EvalR.whileFalse` and {name}`Com.EvalR.whileTrue`; the others
 are contradictory.
 
-- Suppose `st =[ while (~b) {~c} ]=> st'` is proved using rule
-  `Com.EvalR.whileFalse`.  Then by assumption `b.eval st = false`. But
+- Suppose `st =[ while (b) {c} ]=> st'` is proved using rule
+  {name}`Com.EvalR.whileFalse`.  Then by assumption `b.eval st = false`. But
   this contradicts the assumption that `b` is equivalent to
   `true`.
 
-- Suppose `st =[ while (~b) {~c} ]=> st'` is proved using rule
-  `Com.EvalR.whileTrue`.  We must have:
+- Suppose `st =[ while (b) {c} ]=> st'` is proved using rule
+  {name}`Com.EvalR.whileTrue`.  We must have:
 
   1. `b.eval st = true`, and
   2. there is some `st₀` such that `st =[ c ] => st₀` and
-     `st₀ =[ while (~b) {~c} ]=> st'`.
+     `st₀ =[ while (b) {c} ]=> st'`.
   3. Also, we are given an induction hypothesis saying that
-     `st₀ =[ while (~b) {~c} ]=> st'` leads to a contradiction,
+     `st₀ =[ while (b) {c} ]=> st'` leads to a contradiction,
 
   We obtain a contradiction by 2 and 3.
 ::::
 
 ```lean
-theorem while_true_nonterm {b : Bexp} {c : Com} {st st' : State} (hb : b.Equiv (bexp {true})) :
-    ¬ st =[ while (~b) {~c} ]=> st' := by
+theorem while_true_nonterm {b : Bexp} {c : Com} {st st' : State} (hb : b ≃ bexp {true}) :
+    ¬ st =[ while (b) {c} ]=> st' := by
   workinclass!
     intro contra
-    generalize heq : (imp {while (~b) {~c}}) = com at contra
+    generalize heq : (imp {while (b) {c}}) = com at contra
     induction contra with
-    | @whileFalse b' s0 c0 hb' =>
+    | whileFalse hb' =>
       injection heq with hbeq hceq
       subst hbeq
-      rw [Bexp.equiv_def] at hb
-      simp [hb] at hb'
-    | @whileTrue s0 s0' s0'' b' c0 hb' hc' hwhile ih1 ih2 =>
+      simp_all -- hb and hb' are contradictory
+    | whileTrue hb' hc' hwhile ih1 ih2 =>
       exact ih2 heq
     | skip | asgn | seq | ifTrue | ifFalse =>
-      contradiction -- heq says that different commands are equal
+      contradiction -- `heq` says that different commands are equal
 ```
 :::::exercise (rating := 2) (name := "while_true_nonterm_informal") (manual:= true)
 Explain what the lemma `while_true_nonterm` means in English.
 :::::
+
 :::::exercise (rating := 2) (name := "while_true")
-Prove the following theorem. _Hint_: You'll want to use
-`while_true_nonterm` here.
+Prove the following theorem.
+_Hint_: You'll want to use `while_true_nonterm` here.
 
 ```lean
-theorem while_true {b : Bexp} {c : Com} (hb : b.Equiv (bexp {true})) :
-    (imp {while (~b) {~c}}).Equiv
-    (imp {while (true) {skip}}) := by
+theorem while_true {b : Bexp} {c : Com} (hb : b ≃ bexp {true}) :
+    imp {while (b) {c}} ≃ imp {while (true) {skip}} := by
   solution!
     rw [equiv_def]
     intro st st'
@@ -444,11 +426,11 @@ interest!
 
 ```lean
 theorem loop_unrolling {b : Bexp} {c : Com} :
-    (imp {while (~b) {~c}}).Equiv
-    (imp {
-      if (~b) {~c} else {skip};
-      while (~b) {~c}
-    }) := by
+    imp { while (b) {c} } ≃
+    imp {
+      if (b) {c} else {skip};
+      while (b) {c}
+    } := by
   workinclass!
     rw [equiv_def]
     intro st st'
@@ -472,9 +454,28 @@ theorem loop_unrolling {b : Bexp} {c : Com} :
           inversion hc
           exact h2
 ```
-:::dev "Sati (satiscugcat)"
-Leaving out optional exercise `seq_assoc` for now.
-:::
+
+:::::full
+::::exercise (rating := 2) (name := "seq_assoc") (optional:= true)
+```lean
+theorem seq_assoc {c₁ c₂ c₃ : Com} :
+  imp {~(imp {c₁; c₂}); c₃} ≃ imp {c₁; c₂; c₃} := by
+    solution!
+      intro st₁ st₂
+      constructor <;> intro h
+      · inversion h with
+        | seq h₁ h₂ =>
+            inversion h₁
+            apply EvalR.seq; assumption
+            apply EvalR.seq <;> assumption
+      · inversion h with
+        | seq h₁ h₂ =>
+            inversion h₂
+            apply EvalR.seq <;> try assumption
+            apply EvalR.seq <;> assumption
+```
+::::
+:::::
 
 ::::full
 Proving program properties involving assignments is one place
@@ -485,8 +486,7 @@ in handy.
 
 ```lean
 theorem identity_assignment {X : Ident} :
-    (imp {X := X}).Equiv
-    (imp {skip}) := by
+    imp { X := X } ≃ imp { skip } := by
   rw [equiv_def]
   intro st st'
   constructor
@@ -498,18 +498,16 @@ theorem identity_assignment {X : Ident} :
       exact Com.EvalR.skip
   · intro h
     inversion h
-    suffices st =[ X := X ]=> X →ₜ st[X] ; st by
-      simp only [TotalMap.update_same] at this
-      exact this
-    apply Com.EvalR.asgn
-    simp
+    have h' : st =[ X := X ]=> X →ₜ st[X] ; st := by
+      apply Com.EvalR.asgn
+      simp
+    simp_all [TotalMap.update_same]
 ```
 
 :::::exercise (rating := 2) (name := "assign_equiv")
 ```lean
-theorem assign_equiv {X : Ident} {a : Aexp} (ha : Aexp.Equiv (aexp {X}) a) :
-    (imp {skip}).Equiv
-    (imp {X := ~a}) := by
+theorem assign_equiv {X : Ident} {a : Aexp} (ha : aexp { X } ≃ a) :
+    imp { skip } ≃ imp { X := a } := by
   solution!
     rw [equiv_def]
     rw [Aexp.equiv_def] at ha
@@ -517,11 +515,10 @@ theorem assign_equiv {X : Ident} {a : Aexp} (ha : Aexp.Equiv (aexp {X}) a) :
     constructor
     · intro h
       inversion h
-      suffices st =[ X := ~a ]=> X →ₜ st[X]; st by
-        simp only [TotalMap.update_same] at this
-        exact this
-      apply Com.EvalR.asgn
-      simp [← ha]
+      have h' : st =[ X := ~a ]=> X →ₜ st[X]; st := by
+        apply Com.EvalR.asgn
+        simp [← ha]
+      simp_all [← ha]
     · intro h
       inversion h with
       | asgn n h =>
@@ -531,9 +528,95 @@ theorem assign_equiv {X : Ident} {a : Aexp} (ha : Aexp.Equiv (aexp {X}) a) :
 ```
 :::::
 
-:::dev "Sati (satiscugcat)"
-Leaving out optional exercise `equiv_classes` for now.
-:::
+:::::full
+::::exercise (rating := 2) (name := "equiv_classes") (manual:= true) (optional := true)
+Given the following programs, group together those that are
+equivalent in Imp. Your answer should be given as a list of lists,
+where each sub-list represents a group of equivalent programs. For
+example, if you think programs (a) through (h) are all equivalent
+to each other, but not to (i), your answer should look like this:
+
+```
+[ [progA, progB, progC, progD, progE, progF, progG, progH], [progI] ]
+```
+
+Write down your answer below in the definition of  `equiv_classes`
+
+```lean
+def progA : Com :=
+  imp {
+    while (X > 0) {
+       X := X + 1
+    }
+  }
+
+def progB : Com :=
+  imp {
+    if (X = 0) {
+       X := X + 1;
+       Y := 1
+     } else {
+       Y := 0
+     };
+     X := X - Y;
+     Y := 0
+  }
+
+def progC : Com :=
+  imp { skip }
+
+def progD : Com :=
+  imp {
+    while (X ≠ 0) {
+       X := (X * Y) + 1
+    }
+  }
+
+def progE : Com :=
+  imp { Y := 0 }
+
+def progF : Com :=
+  imp {
+    Y := X + 1;
+    while (X ≠ Y) {
+      Y := X + 1
+    }
+  }
+
+def progG : Com :=
+  imp {
+    while (true) {
+      skip
+    }
+  }
+
+def progH : Com :=
+  imp {
+    while (X ≠ X) {
+      X := X + 1
+    }
+  }
+
+def progI : Com :=
+  imp {
+    while (X ≠ Y) {
+      X := Y + 1
+    }
+  }
+```
+
+```lean
+def equiv_classes : List (List Com) :=
+-- SOLUTION
+  [ [progA, progD] ,
+    [progB, progE] ,
+    [progC, progH] ,
+    [progF, progG] ,
+    [progI] ]
+-- END SOLUTION
+```
+::::
+:::::
 
 # Properties of Behavior Equivalence
 
@@ -544,80 +627,39 @@ We next consider some fundamental properties of program equivalence.
 ## Behavioral Equivalence is an Equivalence
 
 ::::full
-First, let's verify that the equivalences on `Aexp`s, `Bexp`s, and
-`Com`s really are _equivalences_ -- ie, that they are reflexive,
+First, let's verify that the equivalences on {name}`Aexp`s, {name}`Bexp`s, and
+{name}`Com`s really are _equivalences_ - ie, that they are reflexive,
 symmetric, and transitive. These proofs are all easy.
 ::::
 
 ```lean
 end Com
 
-theorem Aexp.equiv_refl (a : Aexp) : a.Equiv a := by
-  rw [equiv_def]
-  intro st
-  rfl
+theorem Aexp.equiv_refl (a : Aexp) : a ≃ a := by simp_all
+theorem Aexp.equiv_symm {a₁ a₂ : Aexp} (h : a₁ ≃ a₂) : a₂ ≃ a₁ := by simp_all
+theorem Aexp.equiv_trans {a₁ a₂ a₃ : Aexp} (h₁ : a₁ ≃ a₂) (h₂ : a₂ ≃ a₃) : a₁ ≃ a₃ := by simp_all
+
+theorem Bexp.equiv_refl {b : Bexp} : b ≃ b := by simp_all
+theorem Bexp.equiv_symm {b₁ b₂ : Bexp} (h : b₁ ≃ b₂) : b₂ ≃ b₁ := by simp_all
+theorem Bexp.equiv_trans {b₁ b₂ b₃ : Bexp} (h₁ : b₁ ≃ b₂) (h₂ : b₂ ≃ b₃) : b₁ ≃ b₃ := by simp_all
+
+theorem Com.equiv_refl {c : Com} : c ≃ c := by simp_all
+theorem Com.equiv_symm {c₁ c₂ : Com} (h : c₁ ≃ c₂) : c₂ ≃ c₁ := by simp_all
+theorem Com.equiv_trans {c₁ c₂ c₃ : Com} (h₁ : c₁ ≃ c₂) (h₂ : c₂ ≃ c₃) : c₁ ≃ c₃ := by simp_all
 ```
+
+::::full
+Lean has a standard library definition for relations that are equivalences, unsurprisingly called
+{name}`Equivalence`. To show that a relation is an {name}`Equivalence`,
+one needs only supply proofs of the three properties above:
 
 ```lean
-theorem Aexp.equiv_symm {a₁ a₂ : Aexp} (h : a₁.Equiv a₂) : a₂.Equiv a₁ := by
-  rw [equiv_def] at h ⊢
-  intro st
-  rw [h]
+theorem Com.equiv_equivalence : Equivalence Com.Equiv where
+  refl := @Com.equiv_refl
+  symm := Com.equiv_symm
+  trans := Com.equiv_trans
 ```
-
-```lean
-theorem Aexp.equiv_trans {a₁ a₂ a₃ : Aexp} (h₁ : a₁.Equiv a₂) (h₂ : a₂.Equiv a₃) :
-    a₁.Equiv a₃ := by
-  rw [equiv_def] at h₁ h₂ ⊢
-  intro st
-  rw [h₁, h₂]
-```
-
-
-```lean
-theorem Bexp.equiv_refl {b : Bexp} : b.Equiv b := by
-  rw [equiv_def]
-  intro st
-  rfl
-```
-
-```lean
-theorem Bexp.equiv_symm {b₁ b₂ : Bexp} (h : b₁.Equiv b₂) : b₂.Equiv b₁ := by
-  rw [equiv_def]
-  intro st
-  rw [h]
-```
-
-```lean
-theorem Bexp.equiv_trans {b₁ b₂ b₃ : Bexp} (h₁ : b₁.Equiv b₂) (h₂ : b₂.Equiv b₃) :
-    b₁.Equiv b₃ := by
-  rw [equiv_def]
-  intro st
-  rw [h₁, h₂]
-```
-
-
-```lean
-theorem Com.equiv_refl {c : Com} : c.Equiv c := by
-  rewrite [equiv_def]
-  intro st st'
-  rfl
-```
-
-```lean
-theorem Com.equiv_symm {c₁ c₂ : Com} (h : c₁.Equiv c₂) : c₂.Equiv c₁ := by
-  rw [equiv_def] at h ⊢
-  intro st st'
-  rw [h]
-```
-
-```lean
-theorem Com.equiv_trans {c₁ c₂ c₃ : Com} (h₁ : c₁.Equiv c₂) (h₂ : c₂.Equiv c₃) :
-    c₁.Equiv c₃ := by
-  rw [equiv_def] at h₁ h₂ ⊢
-  intro st st'
-  rw [h₁, h₂]
-```
+::::
 
 ## Behavioral Equivalence is a Congruence
 
@@ -627,14 +669,14 @@ Less obviously, behavioral equivalence is also a _congruence_.
 That is, the equivalence of two subprograms implies the
 equivalence of the larger programs in which they are embedded:
 
-             aequiv a a'
+              a ≃ a'
      -------------------------
-     cequiv (x := a) (x := a')
+        (x := a) ≃ (x := a')
 
-          cequiv c1 c1'
-          cequiv c2 c2'
+            c₁ ≃ c₁'
+            c₂ ≃ c₂'
      --------------------------
-     cequiv (c1;c2) (c1';c2')
+      (c₁ ; c₂) ≃ (c₁' ; c₂')
 
 ... and so on for the other forms of commands.
 
@@ -651,16 +693,15 @@ properties are important in the following section (in the proof of
 us to replace a small part of a large program with an equivalent
 small part and know that the whole large programs are equivalent
 _without_ doing an explicit proof about the parts that didn't
-change -- i.e., the "proof burden" of a small change to a large
+change - i.e., the "proof burden" of a small change to a large
 program is proportional to the size of the change, not the
 program!
 ::::
 
 
 ```lean
-theorem Com.congruence_asgn {x : Ident} {a a' : Aexp} (ha : a.Equiv a') :
-    (imp {x := ~a}).Equiv
-    (imp {x := ~a'}) := by
+theorem Com.congruence_asgn {x : Ident} {a a' : Aexp} (ha : a ≃ a') :
+    imp {x := a} ≃ imp {x := a'} := by
   rw [equiv_def]
   intro st st'
   constructor <;>
@@ -669,8 +710,7 @@ theorem Com.congruence_asgn {x : Ident} {a a' : Aexp} (ha : a.Equiv a') :
     | asgn n h =>
       subst h
       apply Com.EvalR.asgn
-      rw [Aexp.equiv_def] at ha
-      rw [ha]
+      simp_all
 ```
 
 ::::full
@@ -679,49 +719,48 @@ since it requires induction.
 
 _Theorem_: Equivalence is a congruence for `while` -- that is, if
 `b` is equivalent to `b'` and `c` is equivalent to `c'`, then
-`while (~b) {~c}` is equivalent to `while (~b') {~c'}`.
+`while (b) {c}` is equivalent to `while (b') {c'}`.
 
 _Proof_: Suppose `b` is equivalent to `b'` and `c` is
 equivalent to `c'`.  We must show, for every `st` and `st'`, that
-`st =[ while (~b) {~c} ]=> st'` iff `st = while (~b') {~c'}
-]=> st'`.  We consider the two directions separately.
+`st =[ while (b) {c} ]=> st'` iff `st = while (b') {c'}]=> st'`.
+We consider the two directions separately.
 
-  - (`->`) We show that `st =[ while (~b) {~c} ]=> st'` implies
-    `st =[ while (~b') {~c'} ]=> st'`, by induction on a
-    derivation of `st =[ while (~b) {~c} ]=> st'`.  The only
+  - (`→`) We show that `st =[ while (b) {c} ]=> st'` implies
+    `st =[ while (b') {c'} ]=> st'`, by induction on a
+    derivation of `st =[ while (b) {c} ]=> st'`.  The only
     nontrivial cases are when the final rule in the derivation is
-    `Com.EvalR.whileFalse` or `Com.EvalR.whileTrue`.
+    {name}`Com.EvalR.whileFalse` or {name}`Com.EvalR.whileTrue`.
 
-      - `Com.EvalR.whileFalse`: In this case, the form of the rule gives us
-        `beval st b = false` and `st = st'`.  But then, since
-        `b` and `b'` are equivalent, we have `beval st b' =false`,
-        and `Com.EvalR.whileFalse` applies, giving us
-        `st =[ while (~b') {~c'} ]=> st'`, as required.
+      - {name}`Com.EvalR.whileFalse`: In this case, the form of the rule gives us
+        `b.eval st = false` and `st = st'`.  But then, since
+        `b` and `b'` are equivalent, we have `b'.eval st = false`,
+        and {name}`Com.EvalR.whileFalse` applies, giving us
+        `st =[ while (b') {c'} ]=> st'`, as required.
 
-      - `Com.EvalR.whileTrue`: The form of the rule now gives us `beval st b = true`,
-        with `st =[ c ]=> st'0` and `st'0 =[ while {~b} {~c} ]=> st'`
-        for some state `st'0`, with the
-        induction hypothesis `st'0 =[ while (~b') {~c'} ]=> st'`.
+      - {name}`Com.EvalR.whileTrue`: The form of the rule now gives us `b.eval st = true`,
+        with `st =[ c ]=> st'₀` and `st'₀ =[ while {b} {c} ]=> st'`
+        for some state `st'₀`, with the
+        induction hypothesis `st'₀ =[ while (b') {c'} ]=> st'`.
 
         Since `c` and `c'` are equivalent, we know that `st =[ c']=> st'0`.
         And since `b` and `b'` are equivalent,
-        we have `beval st b' = true`.  Now `Com.EvalR.whileTrue` applies,
-        giving us `st =[ while (~b') {~c'} ]=> st'`, as
+        we have `b'.eval st = true`.  Now {name}`Com.EvalR.whileTrue` applies,
+        giving us `st =[ while (b') {c'} ]=> st'`, as
         required.
 
-  - (`<-`) Similar.
+  - (`←`) Similar.
 ::::
 
 ```lean
-theorem Com.congruence_while {b b' : Bexp} {c c' : Com} (hb : b.Equiv b') (hc : c.Equiv c') :
-    (imp {while (~b) {~c}}).Equiv
-    (imp {while (~b') {~c'}}) := by
+theorem Com.congruence_while {b b' : Bexp} {c c' : Com} (hb : b ≃ b') (hc : c ≃ c') :
+    imp {while (b) {c}} ≃ imp {while (b') {c'}} := by
   workinclass!
     rw [equiv_def]
     intro st st'
     constructor
     · intro h
-      generalize heq : (imp {while (~b) {~c}}) = com at h
+      generalize heq : (imp {while (b) {c}}) = com at h
       induction h with
       | whileFalse hb' =>
         injection heq with hbeq hceq
@@ -729,7 +768,7 @@ theorem Com.congruence_while {b b' : Bexp} {c c' : Com} (hb : b.Equiv b') (hc : 
         apply Com.EvalR.whileFalse
         rw [← hb]
         exact hb'
-      | @whileTrue st₁ st₂ st₃ b₂ c₂ hb' hc' hwhile _ ih2 =>
+      | whileTrue hb' hc' hwhile _ ih2 =>
         injection heq with beq ceq
         subst beq ceq
         rw [hb] at hb'
@@ -748,7 +787,7 @@ theorem Com.congruence_while {b b' : Bexp} {c c' : Com} (hb : b.Equiv b') (hc : 
         apply Com.EvalR.whileFalse
         rw [hb]
         exact hb'
-      | @whileTrue st₁ st₂ st₃ b₂ c₂ hb' hc' hwhile _ ih2 =>
+      | whileTrue hb' hc' hwhile _ ih2 =>
         injection heq with beq ceq
         subst beq ceq
         rw [← hb] at hb'
@@ -761,59 +800,60 @@ theorem Com.congruence_while {b b' : Bexp} {c c' : Com} (hb : b.Equiv b') (hc : 
 ```
 :::::exercise (rating := 3) (name := "Com.congruence_seq") (optional := true)
 ```lean
-theorem Com.congruence_seq {c1 c1' c2 c2' : Com} (hc1 : c1.Equiv c1') (hc2 : c2.Equiv c2') :
-    (imp {~c1 ; ~c2}).Equiv (imp {~c1' ; ~c2'}) := by
+theorem Com.congruence_seq {c₁ c₁' c₂ c₂' : Com} (hc₁ : c₁ ≃ c₁') (hc₂ : c₂ ≃ c₂') :
+    imp {c₁ ; ~c₂} ≃ imp {c₁' ; c₂'} := by
   solution!(
     intro st st'
     constructor
     · intro h
       inversion h with
-      | seq hc1' hc2' =>
-        rw [equiv_def] at hc1
-        rw [equiv_def] at hc2
-        exact Com.EvalR.seq (hc1.mp hc1') (hc2.mp hc2')
+      | seq hc₁' hc₂' =>
+        rw [equiv_def] at hc₁
+        rw [equiv_def] at hc₂
+        exact Com.EvalR.seq (hc₁.mp hc₁') (hc₂.mp hc₂')
     · intro h
       inversion h with
-      | seq hc1' hc2' =>
-        rw [equiv_def] at hc1
-        rw [equiv_def] at hc2
-        exact Com.EvalR.seq (hc1.mpr hc1') (hc2.mpr hc2')
+      | seq hc₁' hc₂' =>
+        rw [equiv_def] at hc₁
+        rw [equiv_def] at hc₂
+        exact Com.EvalR.seq (hc₁.mpr hc₁') (hc₂.mpr hc₂')
   )
 ```
 :::::
 
 :::::exercise (rating := 3) (name := "Com.congruence_if")
 ```lean
-theorem Com.congruence_if {b b' : Bexp} {c1 c1' c2 c2' : Com} (hb : b.Equiv b') (hc1 : c1.Equiv c1') (hc2 : c2.Equiv c2') :
-    (imp {if (~b) {~c1} else {~c2}}).Equiv
-    (imp {if (~b') {~c1'} else {~c2'}}) := by
+theorem Com.congruence_if {b b' : Bexp} {c₁ c₁' c₂ c₂' : Com}
+   (hb : b ≃ b') (hc₁ : c₁ ≃ c₁') (hc₂ : c₂ ≃ c₂') :
+    (imp {if (b) {c₁} else {c₂}}).Equiv
+    (imp {if (b') {c₁'} else {c₂'}}) := by
   solution!(
     intro st st'
     constructor
     · intro h
       inversion h with
-      | ifTrue hb' hc1' =>
+      | ifTrue hb' hc₁' =>
         rw [hb] at hb'
         apply Com.EvalR.ifTrue <;> try assumption
-        · rw [equiv_def] at hc1
-          exact (hc1.mp hc1')
-      | ifFalse hb' hc2' =>
+        · rw [equiv_def] at hc₁
+          exact (hc₁.mp hc₁')
+      | ifFalse hb' hc₂' =>
         rw [hb] at hb'
         apply Com.EvalR.ifFalse <;> try assumption
-        · rw [equiv_def] at hc2
-          exact (hc2.mp hc2')
+        · rw [equiv_def] at hc₂
+          exact (hc₂.mp hc₂')
     · intro h
       inversion h with
-      | ifTrue hb' hc1' =>
+      | ifTrue hb' hc₁' =>
         rw [← hb] at hb'
         apply Com.EvalR.ifTrue <;> try assumption
-        · rw [equiv_def] at hc1
-          exact (hc1.mpr hc1')
-      | ifFalse hb' hc2' =>
+        · rw [equiv_def] at hc₁
+          exact (hc₁.mpr hc₁')
+      | ifFalse hb' hc₂' =>
         rw [← hb] at hb'
         apply Com.EvalR.ifFalse <;> try assumption
-        · rw [equiv_def] at hc2
-          exact (hc2.mpr hc2')
+        · rw [equiv_def] at hc₂
+          exact (hc₂.mpr hc₂')
   )
 ```
 :::::
@@ -824,20 +864,19 @@ For example, here are two programs and a proof of their equivalence using their 
 
 ```lean
 example :
-    (imp {X := 0; if (X = 0) {Y := 0} else {Y := 42}}).Equiv
-    (imp {X := 0; if (X = 0) {Y := X - X} else {Y := 42}}) := by
+    imp {X := 0; if (X = 0) {Y := 0} else {Y := 42}} ≃
+    imp {X := 0; if (X = 0) {Y := X - X} else {Y := 42}} := by
   apply Com.congruence_seq
   · apply Com.equiv_refl
   · apply Com.congruence_if
     · apply Bexp.equiv_refl
     · apply Com.congruence_asgn
-      rw [Aexp.equiv_def]
       simp
     · apply Com.equiv_refl
 ```
 
 :::::exercise (rating := 3) (name := "not_congr") (level := Advanced) (manual := true)
-We've shown that the `Com.Equiv` relation is both an equivalence and
+We've shown that the {name}`Com.Equiv` relation is both an equivalence and
 a congruence on commands.  Can you think of a relation on commands
 that is an equivalence but _not_ a congruence?  Write down the
 relation (formally), together with an informal sketch of a proof
@@ -856,23 +895,28 @@ but there are many others.
 
 ```lean
 def Aexp.TransSound (trans : Aexp → Aexp) : Prop :=
-  ∀ (a : Aexp), a.Equiv (trans a)
+  ∀ (a : Aexp), a ≃ (trans a)
 
+@[simp]
 theorem Aexp.transSound_def {trans : Aexp → Aexp} :
-    TransSound trans ↔ ∀ (a : Aexp), a.Equiv (trans a) := by rfl
+    TransSound trans ↔ ∀ (a : Aexp), a ≃ (trans a) := by rfl
 
 def Bexp.TransSound (trans : Bexp → Bexp) : Prop :=
-  ∀ (b : Bexp), b.Equiv (trans b)
+  ∀ (b : Bexp), b ≃ (trans b)
 
+@[simp]
 theorem Bexp.transSound_def {trans : Bexp → Bexp} :
-    TransSound trans ↔ ∀ (b : Bexp), b.Equiv (trans b) := by rfl
+    TransSound trans ↔ ∀ (b : Bexp), b ≃ (trans b) := by rfl
 
 def Com.TransSound (trans : Com → Com) : Prop :=
-  ∀ (c : Com), c.Equiv (trans c)
+  ∀ (c : Com), c ≃ (trans c)
 
+@[simp]
 theorem Com.transSound_def {trans : Com → Com} :
-    TransSound trans ↔ ∀ (c : Com), c.Equiv (trans c) := by rfl
+    TransSound trans ↔ ∀ (c : Com), c ≃ (trans c) := by rfl
 ```
+
+
 ## The Constant-Folding Transformation
 
 ::::full
@@ -907,9 +951,9 @@ theorem Aexp.foldConstants_id (x : Ident) : (Aexp.id x).foldConstants = .id x :=
 
 theorem Aexp.foldConstants_cases (a₁ a₂ : Aexp) :
     (∃ n₁ n₂, a₁.foldConstants = .num n₁ ∧ a₂.foldConstants = .num n₂) ∨
-    (aexp {~a₁ + ~a₂}).foldConstants = (aexp {~a₁.foldConstants + ~a₂.foldConstants}) ∧
-    (aexp {~a₁ - ~a₂}).foldConstants = (aexp {~a₁.foldConstants - ~a₂.foldConstants}) ∧
-    (aexp {~a₁ * ~a₂}).foldConstants = (aexp {~a₁.foldConstants * ~a₂.foldConstants}) := by
+    (aexp {a₁ + a₂}).foldConstants = (aexp {~a₁.foldConstants + ~a₂.foldConstants}) ∧
+    (aexp {a₁ - a₂}).foldConstants = (aexp {~a₁.foldConstants - ~a₂.foldConstants}) ∧
+    (aexp {a₁ * a₂}).foldConstants = (aexp {~a₁.foldConstants * ~a₂.foldConstants}) := by
   cases ha₁ : a₁.foldConstants with
   | num n₁ =>
     cases ha₂ : a₂.foldConstants with
@@ -946,10 +990,11 @@ example : (aexp { X - ((0 * 6) + Y) }).foldConstants = (aexp { X - (0 + Y) }) :=
 ```
 
 ::::full
-Not only can we lift `Aexp.foldConstants` to `Bexp` in the `Bexp.eq`, `Bexp.neq`, and
-`Bexp.le` cases, we can also look for constant _boolean_ expressions and evaluate them
-in place as well.
+Not only can we lift {name}`Aexp.foldConstants` to {name}`Bexp` in the {name}`Bexp.eq`,
+{name}`Bexp.neq`, and {name}`Bexp.le` cases, we can also look for constant
+_boolean_ expressions and evaluate them in place as well.
 ::::
+
 ```lean
 def Bexp.foldConstants (b : Bexp) : Bexp :=
   match b with
@@ -1025,7 +1070,7 @@ theorem Bexp.foldConstants_binary (b₁ : Bexp) (b₂ : Bexp) :
     | _ => simp [foldConstants, hb₁, hb₂]
   | _ => simp [foldConstants, hb₁]
 
-  
+
 ```
 ```lean
 example : (bexp { true ∧ ¬( false ∧ true) }).foldConstants = (bexp { true }) := by rfl
@@ -1036,24 +1081,24 @@ example : (bexp { (X = Y) ∧ ( 0 = (2 - (1 + 1))) }).foldConstants = (bexp { (X
 To fold constants in a command, we simply apply the
 appropriate folding functions on all embedded expressions.
 ::::
+
 ```lean
 def Com.foldConstants (c : Com) : Com :=
   match c with
   | imp { skip } => imp { skip }
   | imp { x := ~a } => imp { x := ~a.foldConstants }
-  | imp { ~c₁ ; ~c₂ } =>  imp { ~c₁.foldConstants ; ~c₂.foldConstants }
-  | imp { if (~b) {~c₁} else {~c₂}} =>
+  | imp { c₁ ; c₂ } =>  imp { c₁.foldConstants ; c₂.foldConstants }
+  | imp { if (b) { c₁ } else { c₂ }} =>
     match b.foldConstants with
     | bexp { true } => c₁.foldConstants
     | bexp { false } => c₂.foldConstants
-    | b' => imp { if (~b') {~c₁.foldConstants} else {~c₂.foldConstants}}
-  | imp { while (~b) {~c}} =>
+    | b' => imp { if (b') {c₁.foldConstants} else { c₂.foldConstants}}
+  | imp { while (b) {c}} =>
     match b.foldConstants with
     | bexp { true } => imp { while (true) { skip }}
     | bexp { false } => imp { skip }
-    | b' => imp { while (~b') {~c.foldConstants}}
-```
-```lean
+    | b' => imp { while (b') {c.foldConstants}}
+
 example :
   (imp {
     X := 4 + 5;
@@ -1070,7 +1115,9 @@ example :
     while (Y = 0) {X := X+1}
   }) := by rfl
 ```
+
 ## Soundness of Constant Folding
+
 ::::full
 Now we need to show that what we've done is correct.
 ::::
@@ -1078,37 +1125,1422 @@ Now we need to show that what we've done is correct.
 ::::full
 Here's the proof for arithmetic expressions.
 ::::
+
 ```lean
 theorem Aexp.foldConstants_sound : TransSound foldConstants := by
-  rw [transSound_def]
-  intro a
-  rw [equiv_def]
-  intro st
+  intro a st
   induction a with
   | num n | id x => rfl
   | _ a₁ a₂ _ _ =>
     cases foldConstants_cases a₁ a₂ with
     | inl h =>
       obtain ⟨n₁, n₂, h₁, h₂⟩ := h
-      rw [foldConstants]
-      simp_all
+      simp_all [foldConstants]
     | inr h =>
       simp_all
+```
 
--- Golfed version with `fun_induction`
+An equivalent version using the {tactic}`fun_induction` tactic would look simpler:
+```lean
 theorem Aexp.foldConstants_sound' : TransSound foldConstants := by
-  rw [transSound_def]
-  intro a
-  rw [equiv_def]
-  intro st
+  intro a st
   fun_induction foldConstants a <;> simp_all
 ```
-:::dev "Sati (satiscugcat)"
+
+:::::full
+::::exercise (rating := 3) (manual := true) (optional := true) (name := "fold_bexp_Eq_informal")
+Here is an informal proof of the `eq` case of the soundness
+argument for boolean expression constant folding.  Read it
+carefully and compare it to the formal proof that follows.  Then
+fill in the `le` case of the formal proof (without looking at the
+`eq` case, if possible).
+
+_Theorem_: The constant folding function for booleans,
+`fold_constants_bexp`, is sound.
+
+_Proof_: We must show that `b` is equivalent to `fold_constants_bexp b`,
+for all boolean expressions `b`.  Proceed by induction on `b`.  We
+show just the case where `b` has the form `a₁ = a₂`.
+
+In this case, we must show
 ```
-NOT PORTED YET - remaining portions of Equiv.v left (apart from the portions explicitly stated so far).
-  - The section on "Program Transformation"
-  - Soundness of (0 + n) Elimination
-  - Extended Exercise: Nondeterministic Imp
-  - Additional Exercises
+(imp { a₁ = a₂ }).eval st = (fold_constants_bexp (imp { a₁ = a₂ })).eval st
+```
+
+There are two cases to consider:
+
+- First, suppose `fold_constants_aexp a₁ = imp { n₁ }` and
+  `fold_constants_aexp a₂ = imp { n₂ }` for some `n₁` and `n₂`.
+
+  In this case, we have
+
+```
+  fold_constants_bexp (imp { a₁ = a₂ }) = if (n₁ = n₂) then imp { true } else imp { false }
+```
+
+  and
+
+```
+(imp {a₁ = a₂}).eval st = a₁.eval st = a₂.eval st.
+```
+
+  By the soundness of constant folding for arithmetic
+  expressions (`fold_constants_aexp_sound`), we know
+
+```
+           a₁.eval st
+         = (fold_constants_aexp a₁).eval st
+         = (imp { n₁ }).eval st
+         = n₁
+```
+
+  and
+
+```
+           a₂.eval st
+         = (fold_constants_aexp a₂).eval st
+         = (imp { n₂ }).eval st
+         = n₂
+```
+
+  so
+
+```
+          imp { a₁ = a₂ }.eval st
+         = (aeval a₁) = (aeval a₂)
+         = n₁ = n₂
+```
+
+      Also, it is easy to see (by considering the cases `n₁ = n₂` and
+      `n₁ ≠ n₂` separately) that
+```
+          (if n₁ = n₂ then (imp { true }) else (imp { false }) ).eval st
+         = if n₁ = n₂ then imp { true }.eval st else imp { false }.eval st
+         = if n₁ = n₂ then true else false
+         = n₁ = n₂
+```
+      So
+```
+           ((imp { a₁ = a₂ })).eval st
+         = n₁ = n₂.
+         = (if n₁ = n₂ then (imp { true }) else (imp { false }) ).eval st,
+```
+       as required.
+
+     - Otherwise, one of `fold_constants_aexp a₁` and
+       `fold_constants_aexp a₂` is not a constant.  In this case, we
+       must show
+```
+           imp { a₁ = a₂ }.eval st
+         = beval st (<{ (fold_constants_aexp a₁) =
+                         (fold_constants_aexp a₂) }>),
+```
+       which, by the definition of {name}`Bexp.eval`, is the same as showing
+```
+           a₁.eval st = a₂.eval st
+         = ((fold_constants_aexp a₁)) =.eval st
+                   ((fold_constants_aexp a₂))..eval st
+```
+       But the soundness of constant folding for arithmetic
+       expressions (`fold_constants_aexp_sound`) gives us
+```
+         a₁ = (fold_constants_aexp a₁).eval st
+         a₂ = (fold_constants_aexp a₂),.eval st
+```
+       completing the case.
+
+```lean
+theorem fold_constants_bexp_sound : Bexp.TransSound Bexp.foldConstants := by
+  sorry
+/- Proof.
+  unfold btrans_sound. intros b. unfold bequiv. intros st.
+  induction b;
+    (* true and false are immediate
+    try reflexivity.
+  - (* BEq
+    simpl.
+    remember (fold_constants_aexp a₁) as a1' eqn:Heqa1'.
+    remember (fold_constants_aexp a₂) as a₂' eqn:Heqa2'.
+    replace a₁.eval st with a1'.eval st by
+       (subst a1'; rewrite <- fold_constants_aexp_sound; reflexivity).
+    replace a₂.eval st with a₂'.eval st by
+       (subst a₂'; rewrite <- fold_constants_aexp_sound; reflexivity).
+    destruct a1'; destruct a₂'; try reflexivity.
+    (* The only interesting case is when both a₁ and a₂
+       become constants after folding
+      simpl. destruct (n = n0); reflexivity.
+  - (* BNeq
+    simpl.
+    remember (fold_constants_aexp a₁) as a1' eqn:Heqa1'.
+    remember (fold_constants_aexp a₂) as a₂' eqn:Heqa2'.
+    replace a₁.eval st with a1'.eval st by
+       (subst a1'; rewrite <- fold_constants_aexp_sound; reflexivity).
+    replace a₂.eval st with a₂'.eval st by
+       (subst a₂'; rewrite <- fold_constants_aexp_sound; reflexivity).
+    destruct a1'; destruct a₂'; try reflexivity.
+    (* The only interesting case is when both a₁ and a₂
+       become constants after folding
+      simpl. destruct (n = n0); reflexivity.
+  - (* BLe
+    (* ADMIT
+    simpl.
+    remember (fold_constants_aexp a₁) as a1' eqn:Heqa1'.
+    remember (fold_constants_aexp a₂) as a₂' eqn:Heqa2'.
+    (* a slightly alternative approach using asserts:
+    assert a₁ = a1'.eval st as H1. {.eval st
+      subst a1'. apply fold_constants_aexp_sound. }
+    assert a₂ = a₂'.eval st as H2. {.eval st
+      subst a₂'. apply fold_constants_aexp_sound. }
+    rewrite H1. rewrite H2.
+    destruct a1'; destruct a₂'; try reflexivity.
+      (* Again, the only interesting case is when both a₁ and a₂
+          become constants after folding
+      simpl. destruct (n ≤ n0); reflexivity.
+    (* /ADMIT
+  - (* BGt
+    (* ADMIT
+    simpl.
+    remember (fold_constants_aexp a₁) as a1' eqn:Heqa1'.
+    remember (fold_constants_aexp a₂) as a₂' eqn:Heqa2'.
+    (* a slightly alternative approach using asserts:
+    assert a₁ = a1'.eval st as H1. {.eval st
+      subst a1'. apply fold_constants_aexp_sound. }
+    assert a₂ = a₂'.eval st as H2. {.eval st
+      subst a₂'. apply fold_constants_aexp_sound. }
+    rewrite H1. rewrite H2.
+    destruct a1'; destruct a₂'; try reflexivity.
+      (* Again, the only interesting case is when both a₁ and a₂
+          become constants after folding
+      simpl. destruct (n ≤ n0); reflexivity.
+    (* /ADMIT
+  - (* BNot
+    simpl. remember (fold_constants_bexp b) as b' eqn:Heqb'.
+    rewrite IHb.
+    destruct b'; reflexivity.
+  - (* BAnd
+    simpl.
+    remember (fold_constants_bexp b₁) as b1' eqn:Heqb1'.
+    remember (fold_constants_bexp b₂) as b2' eqn:Heqb2'.
+    rewrite IHb1. rewrite IHb2.
+    destruct b1'; destruct b2'; reflexivity.
+(* ADMITTED
+Qed.
+(* /ADMITTED  -/
+```
+::::
+:::::
+
+:::::full
+::::exercise (rating := 3) (name := "fold_constants_com_sound") (manual := true) (optional := true)
+Complete the `while` case of the following proof.
+
+```lean
+theorem fold_constants_com_sound : Com.TransSound Com.foldConstants := by sorry
+/- Proof.
+  unfold ctrans_sound. intros c.
+  induction c; simpl.
+  - (* skip  apply refl_cequiv.
+  - (* :=  apply CAsgn_congruence.
+              apply fold_constants_aexp_sound.
+  - (* ;  apply CSeq_congruence; assumption.
+  - (* if
+    assert (bequiv b (fold_constants_bexp b)). {
+      apply fold_constants_bexp_sound. }
+    destruct (fold_constants_bexp b) eqn:Heqb;
+      try (apply CIf_congruence; assumption).
+      (* (If the optimization doesn't eliminate the if, then the
+          result is easy to prove from the IH and
+          [fold_constants_bexp_sound].)
+    + (* b always true
+      apply trans_cequiv with c₁; try assumption.
+      apply if_true; assumption.
+    + (* b always false
+      apply trans_cequiv with c₂; try assumption.
+      apply if_false; assumption.
+  - (* while
+    (* ADMITTED
+    assert (bequiv b (fold_constants_bexp b)).
+    { (* Pf of assertion  apply fold_constants_bexp_sound. }
+    destruct (fold_constants_bexp b) eqn:Heqb;
+      (* Again, the cases where [fold_constants_com] doesn't change
+          the test or don't change the loop body follow from the IH
+          and [fold_constants_bexp_sound]
+      try (apply CWhile_congruence; assumption).
+    + (* b always true
+      apply while_true; assumption.
+    + (* b always false
+      apply while_false; assumption.  Qed.
+(* /ADMITTED -/
+```
+::::
+:::::
+
+# Soundness of (0 + n) Elimination, Redux
+
+:::suppressPreviousHeaderWhenTerse
+:::
+
+:::::full
+
+::::exercise (rating := 4) (name := "optimize0plus_var") (optional := true)
+Recall the definition `optimize0plus` from the {ref "Slang"}[Slang] chapter:
+
+```
+def optimize0plus (a : Aexp) : Aexp :=
+  match a with
+  | num   n          => num n
+  | plus  (num 0) e₂ => optimize0plus e₂
+  | plus  e₁      e₂ => plus  (optimize0plus e₁) (optimize0plus e₂)
+  | minus e₁      e₂ => minus (optimize0plus e₁) (optimize0plus e₂)
+  | mult  e₁      e₂ => mult  (optimize0plus e₁) (optimize0plus e₂)
+```
+
+Note that this function is defined over the old version of `Aexp`s,
+without states.
+
+Write a new version of this function that deals with variables (by
+leaving them alone), plus analogous ones for `Bexp`s and commands:
+
+```
+Aexp.optimize0plus
+Bexp.optimize0plus
+Com.optimize0plus
+```
+
+```lean
+def Aexp.optimize0plus (a : Aexp) : Aexp :=
+-- SOLUTION
+match a with
+| Aexp.num n => Aexp.num n
+| Aexp.id x => Aexp.id x
+| (aexp { 0 + ~a₂ }) => Aexp.optimize0plus a₂
+| (aexp { ~a₁ + ~a₂ }) => (aexp { ~(Aexp.optimize0plus a₁) + ~(Aexp.optimize0plus a₂) })
+| (aexp { ~a₁ - ~a₂ }) => (aexp { ~(Aexp.optimize0plus a₁) - ~(Aexp.optimize0plus a₂) })
+| (aexp { ~a₁ * ~a₂ }) => (aexp { ~(Aexp.optimize0plus a₁) * ~(Aexp.optimize0plus a₂) })
+-- END SOLUTION
+
+def Bexp.optimize0plus (b : Bexp) : Bexp :=
+-- SOLUTION
+  match b with
+  | (bexp { true })        => (bexp { true })
+  | (bexp { false })       => (bexp { false })
+  | (bexp { ~a₁ = ~a₂ })  => (bexp { ~(Aexp.optimize0plus a₁) =  ~(Aexp.optimize0plus a₂) })
+  | (bexp { ~a₁ ≠ ~a₂ })  => (bexp { ~(Aexp.optimize0plus a₁) ≠ ~(Aexp.optimize0plus a₂) })
+  | (bexp { ~a₁ ≤ ~a₂ }) => (bexp { ~(Aexp.optimize0plus a₁) ≤ ~(Aexp.optimize0plus a₂) })
+  | (bexp { ~a₁ > ~a₂ })  => (bexp { ~(Aexp.optimize0plus a₁) >  ~(Aexp.optimize0plus a₂) })
+  | (bexp { ¬ ~b₁ })     => (bexp { ¬ ~(Bexp.optimize0plus b₁) })
+  | (bexp { ~b₁ ∧ ~b₂ }) => (bexp { ~(Bexp.optimize0plus b₁) ∧ ~(Bexp.optimize0plus b₂) })
+-- END SOLUTION
+
+def Com.optimize0plus (c : Com) : Com :=
+-- SOLUTION
+match c with
+| (imp { skip })                     => (imp { skip })
+| (imp { x := ~a })                   => (imp { x := ~(Aexp.optimize0plus a) })
+| (imp { c₁ ; c₂ })                  => imp { ~(Com.optimize0plus c₁) ; ~(Com.optimize0plus c₂) }
+| (imp { if (b) {c₁} else {c₂} }) =>
+    imp { if (~(Bexp.optimize0plus b)) {~(Com.optimize0plus c₁)} else {~(Com.optimize0plus c₂)} }
+| (imp { while (b) {c₁} })         => imp { while (~(Bexp.optimize0plus b))
+                                        {~(Com.optimize0plus c₁)} }
+-- END SOLUTION
+```
+
+```lean
+example :
+    Com.optimize0plus
+       (imp { while (X ≠ 0) { X := 0 + X - 1 } }) =
+    (imp { while (X ≠ 0) { X := X - 1 } }) := by
+  rfl
+```
+
+Prove that these three functions are sound, as we did for
+`foldConstants`.  Make sure you use the congruence lemmas in the
+proof for {name}`Com.optimize0plus` - otherwise it will be _long_!
+
+```lean
+theorem optimize0plus_aexp_sound: Aexp.TransSound Aexp.optimize0plus := by sorry
+/- Proof.
+  (* ADMITTED
+  unfold atrans_sound, aequiv.
+  intros a st.
+  induction a;
+    (* Aexp.num and Aexp.id are immediate by definition
+    try (reflexivity);
+    (* AMinus and AMult are immediate by IH
+    try (simpl; rewrite IHa1; rewrite IHa2; reflexivity).
+  - (* APlus
+    destruct a₁;
+    (* everything but Aexp.num and Aexp.id follow from the IH
+    try (simpl; simpl in IHa1; rewrite IHa1; rewrite IHa2; reflexivity).
+    + (* Aexp.num
+      simpl. rewrite IHa2.
+      destruct n as [| n'].
+      * (* n = 0
+        apply add_0_l.
+      * (* n = S n'
+        simpl. reflexivity.
+    + (* Aexp.id
+      simpl. rewrite IHa2. reflexivity.  Qed.
+(* /ADMITTED -/
+
+theorem optimize0plus_bexp_sound: Bexp.TransSound Bexp.optimize0plus := by sorry
+/-  (* ADMITTED
+  unfold btrans_sound, bequiv.
+  intros b st. induction b; simpl;
+               try reflexivity;
+               try (rewrite IHb1; rewrite IHb2; reflexivity);
+               try (rewrite <- optimize0plus_aexp_sound;
+                    rewrite <- optimize0plus_aexp_sound;
+                    reflexivity).
+  - (* BNot
+    rewrite IHb. reflexivity.  Qed.
+(* /ADMITTED -/
+
+theorem optimize0plus_com_sound: Com.TransSound Com.optimize0plus := by sorry
+/-
+  (* ADMITTED
+  unfold ctrans_sound, cequiv.
+  intros c.
+  induction c;
+  intros st st'; simpl.
+  - (* skip
+    apply refl_cequiv.
+  - (* :=
+    apply CAsgn_congruence.
+    apply optimize0plus_aexp_sound.
+  - (* ;
+    apply CSeq_congruence; unfold cequiv.
+    + apply IHc1.
+    + apply IHc2.
+  - (* if
+    apply CIf_congruence; unfold cequiv.
+    + apply optimize0plus_bexp_sound.
+    + apply IHc1.
+    + apply IHc2.
+  - (* while
+    apply CWhile_congruence; unfold cequiv.
+    + apply optimize0plus_bexp_sound.
+    + apply IHc.  Qed.
+(* /ADMITTED
+(* GRADE_THEOREM 2: optimize0plus_com_sound -/
+```
+
+Finally, let's define a compound optimizer on commands that first
+folds constants (using {name}`Com.foldConstants`) and then eliminates
+`0 + n` terms (using{name}`Com.optimize0plus`).
+
+```lean
+def optimizer (c : Com) := Com.optimize0plus (Com.foldConstants c)
+```
+
+Prove that this optimizer is sound.
+
+```lean
+theorem optimizer_sound : Com.TransSound optimizer := by sorry
+ /- (* ADMITTED
+  unfold ctrans_sound. unfold optimizer.
+  intros c.
+  apply trans_cequiv with (fold_constants_com c).
+  - apply fold_constants_com_sound. -/
+```
+::::
+:::::
+
+# Proving Inequivalence
+
+Next, let's look at some programs that are _not_ equivalent.
+
+Suppose that `c₁` is a command of the form
+
+```
+  X := a₁; Y := a₂
+```
+
+and `c₂` is the command
+
+```
+       X := a₁; Y := a₂'
+```
+
+where `a₂'` is formed by substituting `a₁` for all occurrences
+of `X` in `a₂`.
+
+For example, `c₁` and `c₂` might be:
+
+```
+       c₁  =  (X := 42 + 53;
+               Y := Y + X)
+       c₂  =  (X := 42 + 53;
+               Y := Y + (42 + 53))
+```
+
+Clearly, this _particular_ `c₁` and `c₂` are equivalent.  Is this
+true in general?
+
+:::full
+We will see in a moment that it is not, but it is worthwhile
+to pause, now, and see if you can find a counter-example on your
+own.
+:::
+
+More formally, here is the function that substitutes an arithmetic
+expression `u` for each occurrence of a given variable `x` in
+another expression `a`:
+
+```lean
+def Aexp.subst (x : String) (u : Aexp) (a : Aexp) : Aexp :=
+  match a with
+  | Aexp.num n       =>
+      Aexp.num n
+  | Aexp.id x'       =>
+      if x = x' then u else Aexp.id x'
+  | (aexp { ~a₁ + ~a₂ })  =>
+      (aexp { ~(Aexp.subst x u a₁) + ~(Aexp.subst x u a₂) })
+  | (aexp { ~a₁ - ~a₂ }) =>
+      (aexp { ~(Aexp.subst x u a₁) - ~(Aexp.subst x u a₂) })
+  | (aexp { ~a₁ * ~a₂ })  =>
+      (aexp { ~(Aexp.subst x u a₁) * ~(Aexp.subst x u a₂) })
+
+example :
+  Aexp.subst X (aexp { 42 + 53 })  (aexp { Y + X })
+  = (aexp {  Y + (42 + 53) }) := by rfl
+```
+
+And here is the property we are interested in, expressing the
+claim that commands `c₁` and `c₂` as described above are
+always equivalent.
+
+```lean
+def SubstEquivProperty : Prop := ∀ (x₁ x₂ : String) (a₁ a₂ : Aexp),
+  (imp { x₁ := a₁; x₂ := a₂ }) ≃
+  (imp { x₁ := a₁; x₂ := ~(Aexp.subst x₁ a₁ a₂) })
+```
+
+
+Sadly, the property does _not_ always hold.
+
+Here is a counterexample:
+```
+  X := X + 1; Y := X
+```
+
+If we perform the substitution, we get
+
+```
+  X := X + 1; Y := X + 1
+```
+
+which clearly isn't equivalent.
+
+```lean
+theorem subst_inequiv : ¬ SubstEquivProperty := by sorry
+/-
+Proof.
+  unfold subst_equiv_property.
+  intros Contra.
+
+  (* Here is the counterexample: assuming that [subst_equiv_property]
+     holds allows us to prove that these two programs are
+     equivalent...
+  remember <{ X := X + 1;
+              Y := X }>
+      as c₁.
+  remember <{ X := X + 1;
+              Y := X + 1 }>
+      as c₂.
+  assert (cequiv c₁ c₂) by (subst; apply Contra).
+  clear Contra.
+
+  (* ... allows us to show that the command `c₂` can terminate
+     in two different final states:
+        st1 = (Y →ₜ 1 ; X →ₜ 1)
+        st2 = (Y →ₜ 2 ; X →ₜ 1).
+  remember (Y →ₜ 1 ; X →ₜ 1) as st1.
+  remember (Y →ₜ 2 ; X →ₜ 1) as st2.
+  assert (H1 : empty_st =[ c₁ ]=> st1);
+  assert (H2 : empty_st =[ c₂ ]=> st2);
+  try (subst;
+       apply E_Seq with (st' := (X →ₜ 1));
+       apply E_Asgn; reflexivity).
+  clear Heqc1 Heqc2.
+
+  apply H in H1.
+  clear H.
+
+  (* Finally, we use the fact that evaluation is deterministic
+     to obtain a contradiction.
+  assert (Hcontra : st1 = st2)
+    by (apply (ceval_deterministic c₂ empty_st); assumption).
+  clear H1 H2.
+
+  assert (Hcontra' : st1 Y = st2 Y)
+    by (rewrite Hcontra; reflexivity).
+  subst. discriminate. Qed.
+-/
+```
+
+:::::full
+::::exercise (rating := 4) (name := "better_subst_equiv") (optional := true)
+
+The equivalence we had in mind above was not complete nonsense --
+in fact, it was actually almost right.  To make it correct, we
+just need to exclude the case where the variable `X` occurs in the
+right-hand side of the first assignment statement.
+
+```lean
+inductive VarNotUsedInAexp (x : String) : Aexp → Prop where
+  | num {n : Nat} : VarNotUsedInAexp x (Aexp.num n)
+  | id {y : String} (h : x ≠ y) : VarNotUsedInAexp x (Aexp.id y)
+  | plus {a₁ a₂ : Aexp}
+      (h₁ : VarNotUsedInAexp x a₁)
+      (h₂ : VarNotUsedInAexp x a₂) :
+      VarNotUsedInAexp x ((aexp { ~a₁ + ~a₂ }))
+  | minus {a₁ a₂ : Aexp}
+      (h₁ : VarNotUsedInAexp x a₁)
+      (h₂ : VarNotUsedInAexp x a₂) :
+      VarNotUsedInAexp x ((aexp { ~a₁ - ~a₂ }))
+  | mult {a₁ a₂ : Aexp}
+      (h₁ : VarNotUsedInAexp x a₁)
+      (h₂ : VarNotUsedInAexp x a₂) :
+      VarNotUsedInAexp x ((aexp { ~a₁ * ~a₂ }))
+```
+
+```lean
+theorem Aexp.eval_weakening {x : String} {st : State} {a : Aexp} {ni : Nat}
+  (h : VarNotUsedInAexp x a) :
+  a.eval (x →ₜ ni ; st) = a.eval st := by sorry
+/- Proof.
+  (* ADMITTED
+  intros x st a.
+  induction a; intros nx Hx;
+    (* the binary operators follow from the IH
+    try (simpl; inversion Hx; subst;
+         rewrite IHa1; try assumption;
+         rewrite IHa2; try assumption;
+         reflexivity).
+  - (* Aexp.num
+    reflexivity.
+  - (* Aexp.id
+    inversion Hx; subst. simpl.
+    apply t_update_neq. assumption. Qed.
+  (* /ADMITTED -/
+```
+
+Using `VarNotUsedInAexp`, formalize and prove a correct version
+of `SubstEquivProperty`.
+
+:::solution
+```lean
+theorem aeval_subst {x : String} {st : State} {a₁ a₂ : Aexp}
+  (h : VarNotUsedInAexp x a₁) :
+  a₂.eval (x →ₜ a₁.eval st ; st) = (Aexp.subst x a₁ a₂).eval (x →ₜ a₁.eval st ; st) := by sorry
+/- Proof.
+  intros x st a₁ a₂ Hi.
+  generalize dependent st.
+  induction a₂ as [| x' | | | ]; intros st;
+    (* operator cases follow from the IH
+    try (simpl; rewrite → IHa2_1; rewrite → IHa2_2; reflexivity).
+  - (* Aexp.num
+    reflexivity.
+  - (* Aexp.id
+    unfold Aexp.subst.
+    destruct (String.eqb_spec x x') as [H | H].
+    + (* x = x'
+      subst x'.
+      rewrite aeval_weakening with (a := a₁); try assumption.
+      simpl. rewrite t_update_eq. reflexivity.
+    + (* x ≠ x'
+      reflexivity.  Qed. -/
+
+theorem subst_equiv {x₁ x₂ : String} {a₁ a₂ : Aexp}
+  (h : VarNotUsedInAexp x₁ a₁) :
+  imp { x₁ := a₁; x₂ := a₂ } ≃
+  imp { x₁ := a₁; x₂ := ~(Aexp.subst x₁ a₁ a₂)} := by sorry
+/- Proof.
+  unfold cequiv. intros x₁ x₂ a₁ a₂ Hi.
+  split; intros Hce.
+  ·
+    inversion Hce; subst.
+    apply E_Seq with st'0; try assumption.
+    inversion H4; subst. apply E_Asgn.
+    inversion H1; subst. symmetry. apply aeval_subst.
+    assumption.
+  ·
+    inversion Hce; subst.
+    apply E_Seq with st'0.
+    + assumption.
+    + inversion H4; subst. apply E_Asgn.
+      inversion H1; subst. apply aeval_subst.
+      assumption.  Qed. -/
 ```
 :::
+::::
+:::::
+
+:::::full
+::::exercise (rating := 3) (name := "inequiv_exercise") (manual := true) (optional := true)
+Prove that an infinite loop is not equivalent to `skip`.
+
+```lean
+theorem inequiv_exercise:
+  ¬ (imp { while (true) {skip} } ≃ imp { skip }) := by sorry
+/- Proof.
+  (* ADMITTED
+  intros Contra.
+  assert (~(empty_st =[ while true do skip end ]=> empty_st)) as H.
+  { apply while_true_nonterm. apply refl_bequiv. }
+  apply H.
+  apply (Contra empty_st empty_st).
+  apply E_Skip. Qed.
+(* /ADMITTED -/
+```
+::::
+:::::
+
+# Extended Exercise: Nondeterministic Imp
+
+:::suppressPreviousHeaderWhenTerse
+:::
+
+:::::full
+As we have seen (in theorem `ceval_deterministic` in the `Imp`
+chapter), Imp's evaluation relation is deterministic.  However,
+_non_-determinism is an important part of the definition of many
+real programming languages. For example, in many imperative
+languages (such as C and its relatives), the order in which
+function arguments are evaluated is unspecified: the program
+fragment
+
+```
+  x = 0;
+  f(++x, x)
+```
+
+might call `f` with arguments `(1, 0)` or `(1, 1)`, depending how
+the compiler chooses to order things.  This can be a little
+confusing for programmers, but it gives compiler writers useful
+freedom.
+
+In this exercise, we will extend Imp with a simple
+nondeterministic command and study how this change affects
+program equivalence.  The new command has the syntax `havoc X`,
+where `X` is an identifier. The effect of executing `havoc X` is
+to assign an _arbitrary_ number to the variable `X`,
+nondeterministically. For example, after executing the program:
+
+```
+  havoc Y;
+  Z := Y * 2
+```
+
+the value of `Y` can be any number, while the value of `Z` is
+twice that of `Y` (so `Z` is always even). Note that we are not
+saying anything about the _probabilities_ of the outcomes -- just
+that there are (infinitely) many different outcomes that can
+possibly happen after executing this nondeterministic code.
+
+In a sense, a variable on which we do `havoc` roughly corresponds
+to an uninitialized variable in a low-level language like C.  After
+the `havoc`, the variable holds a fixed but arbitrary number.  Most
+sources of nondeterminism in language definitions are there
+precisely because programmers don't care which choice is made (and
+so it is good to leave it open to the compiler to choose whichever
+will run faster).
+
+We call this new language _Himp_ ("Imp extended with `havoc`").
+
+```lean
+namespace Himp
+```
+
+To formalize Himp, we first add a clause to the definition of
+commands.
+
+```lean
+inductive Com : Type where
+  | skip : Com
+  | asgn : String → Aexp → Com
+  | seq : Com → Com → Com
+  | cond : Bexp → Com → Com → Com
+  | whileDo : Bexp → Com → Com
+  | havoc : String → Com  --  <--- NEW
+```
+:::details "Notation encoding: commands, macro rules"
+```lean
+namespace Com
+
+/-- Assignment -/
+syntax:max "havoc" ppHardSpace ident : imp_com
+
+open Lean
+
+scoped macro_rules
+  | `(imp { $s }) => do
+    let stx ← match s with
+      | `(imp_com| skip) => ``(Com.skip)
+      | `(imp_com| havoc $x:ident) => ``(Com.havoc $x)
+      | `(imp_com| $x:ident) => ``(($x : Com))
+      | `(imp_com| $c₁ ; $c₂) =>
+        ``(Com.seq (imp {$c₁}) (imp {$c₂}))
+      | `(imp_com| $x:ident := $a) =>
+        ``(Com.asgn $x (aexp {$a}))
+      | `(imp_com| if ($b) {$c₁} else {$c₂}) =>
+        ``(Com.cond (bexp {$b}) (imp {$c₁}) (imp {$c₂}))
+      | `(imp_com| while ($b) {$c}) =>
+        ``(Com.whileDo (bexp {$b}) (imp {$c}))
+      | `(imp_com| ~$c) => `(($c : Com))
+      | _ => Macro.throwUnsupported
+    return Imp.Elab.withSourceInfoOf s stx
+
+end Com
+
+open scoped Com
+
+namespace Delab
+open Lean PrettyPrinter Imp.Delab
+
+@[app_unexpander Com.havoc]
+def unexpandComHavoc : Unexpander
+  | `($_ $x:ident) => `(imp { havoc $x:ident })
+  | _ => throw ()
+
+attribute [app_unexpander Com.skip] unexpandComSkip
+attribute [app_unexpander Com.asgn] unexpandComAsgn
+attribute [app_unexpander Com.seq] unexpandComSeq
+attribute [app_unexpander Com.cond] unexpandComCond
+attribute [app_unexpander Com.whileDo] unexpandComWhileDo
+
+end Delab
+```
+
+```lean
+/-- info: imp {havoc X} : Com -/
+#guard_msgs in
+#check imp { havoc X }
+```
+:::
+
+::::exercise (rating := 2) (name := "himp_eval") (manual := true) (optional := true)
+Now, we must extend the operational semantics. We have provided
+a template for the `Com.EvalR` relation below, specifying the big-step
+semantics. What rule(s) must be added to the definition of `Com.EvalR`
+to formalize the behavior of the `havoc` command?
+
+```lean
+inductive Com.EvalR : Com → State → State → Prop where
+  | skip {st : State} : EvalR (imp {skip}) st st
+  | asgn {st : State} {a : Aexp} {n : Nat} {x : Ident} (h : a.eval st = n) :
+      EvalR (imp {x := a}) st (x →ₜ n ; st)
+  | seq {c₁ c₂ : Com} {st st' st'' : State} (h₁ : EvalR c₁ st st') (h₂ : EvalR c₂ st' st'') :
+      EvalR (imp {c₁; c₂}) st st''
+  | ifTrue {st st' : State} {b : Bexp} {c₁ c₂ : Com} (hb : b.eval st = true)
+      (hc : EvalR c₁ st st') :
+      EvalR (imp {if (b) {c₁} else {c₂}}) st st'
+  | ifFalse {st st' : State} {b : Bexp} {c₁ c₂ : Com} (hb : b.eval st = false)
+      (hc : EvalR c₂ st st') :
+      EvalR (imp {if (b) {c₁} else {c₂}}) st st'
+  | whileFalse {b : Bexp} {st : State} {c : Com} (hb : b.eval st = false) :
+      EvalR (imp {while (b) {c}}) st st
+  | whileTrue {st st' st'' : State} {b : Bexp} {c : Com} (hb : b.eval st = true)
+      (hc : EvalR c st st') (hloop : Com.EvalR (imp {while (b) {c}}) st' st'') :
+      EvalR (imp {while (b) {c}}) st st''
+-- SOLUTION
+  | havoc {st : State} {x : String} {n : Nat} :
+      EvalR (imp {havoc x}) st (x →ₜ n ; st)
+-- END SOLUTION
+```
+
+:::details "Notation encoding: commands"
+```lean
+open scoped HasEval
+
+instance : HasEval Com State State where
+  Eval := Com.EvalR
+
+@[simp]
+theorem Com.evalR_eq {c : Com} {st st' : State} :
+    EvalR c st st' ↔ st =[ c ]=> st' := by rfl
+```
+:::
+
+
+As a sanity check, the following claims should be provable for
+your definition:
+
+```lean
+example : ∅ =[ havoc X ]=> (X →ₜ 0) := by
+  constructor
+```
+
+```lean
+example : ∅ =[ skip; havoc Z ]=> (Z →ₜ 42) := by
+  apply Com.EvalR.seq; constructor; constructor
+```
+
+Finally, we repeat the definition of command equivalence from above:
+
+```lean
+def Com.Equiv (c₁ c₂ : Com) : Prop := ∀ (st st' : State),
+  (st =[ c₁ ]=> st') ↔ (st =[ c₂ ]=> st')
+
+instance : Equiv Com where
+  equiv := Com.Equiv
+
+@[simp]
+theorem Com.equiv_notation {c₁ c₂ : Com} : c₁.Equiv c₂ ↔ c₁ ≃ c₂ := by rfl
+@[simp]
+theorem Com.equiv_def {c₁ c₂ : Com} : c₁ ≃ c₂ ↔
+    ∀ {st st' : State}, (st =[ c₁ ]=> st') ↔ (st =[ c₂ ]=> st') := by rfl
+```
+
+Let's apply this definition to prove some nondeterministic
+programs equivalent / inequivalent.
+::::
+:::::
+
+:::::full
+::::exercise (rating := 3) (name := "havoc_swap") (manual := true) (optional := true)
+Are the following two programs equivalent?
+
+```lean
+def pXY := imp { havoc X ; havoc Y }
+
+def pYX := imp { havoc Y; havoc X }
+```
+
+If you think they are equivalent, prove it. If you think they are
+not, prove that.
+
+:::solution
+Note that this is proving something general, considering arbitrary
+x and y, not just the (distinct) string constants X and Y; this is
+why the case distinction is needed.
+
+```lean
+theorem pXY_approx_pYX {x y : String} {st st' : State}
+  (h : st =[ havoc x; havoc y ]=> st') :
+  st =[ havoc y; havoc x ]=> st' := by sorry
+/-  intros x y st st' H.
+  destruct (String.eqb_spec x y) as [Hid | Hid].
+  - (* x = y
+    subst.  assumption.
+  - (* x ≠ y
+    inversion H; subst; clear H.
+    inversion H2; subst; clear H2.
+    inversion H5; subst; clear H5.
+    apply E_Seq with (st' := (y →ₜ n0 ; st)).
+    + constructor.
+    + rewrite t_update_permute.
+      * constructor.
+      * assumption.
+Qed. -/
+```
+:::
+
+```lean
+theorem pXY_cequiv_pYX :
+  (pXY ≃ pYX) ∨ ¬ (pXY ≃ pYX) := by
+/- Hint: You may want to use `update_permute` at some point,
+     in which case you'll probably be left with `X ≠ Y` as a
+     hypothesis. You can use `contradiction to discharge this. -/
+  solution!
+    sorry
+    /- left. intros st st'.
+    split; apply pXY_approx_pYX; reflexivity. -/
+```
+::::
+:::::
+
+:::::full
+::::exercise (rating := 4) (name := "havoc_copy") (optional := true)
+Are the following two programs equivalent?
+
+```lean
+def ptwice :=
+  (imp { havoc X; havoc Y })
+
+def pcopy :=
+  (imp { havoc X; Y := X })
+```
+
+If you think they are equivalent, then prove it. If you think they
+are not, then prove that.  (Hint: You may find the {tactic}`have` tactic
+useful.)
+
+```lean
+theorem ptwice_equiv_pcopy :
+  (ptwice ≃ pcopy) ∨ ¬(ptwice ≃ pcopy) := by sorry
+/- Proof. (* ADMITTED
+  right. intro Hc. unfold cequiv in Hc.
+  assert (empty_st =[ ptwice ]=> (Y →ₜ 1 ; X →ₜ 0)).
+  - apply E_Seq with (X →ₜ 0); constructor.
+  - rewrite Hc in H. inversion H. inversion H2. inversion H5. subst.
+    clear -H13.
+    simpl in H13. rewrite t_update_eq in H13.
+  (* LATER: This trick with [f_equal] is non-evident but highly
+     useful to process contradictory equalities on functions.
+     See [p₃_p₄_inequiv] for a more drastic reduction in code.
+    assert (H0 : n = 1).
+    { apply (f_equal (fun st => st Y)) in H13.
+      apply H13. }
+    assert (H1 : n = 0).
+    { apply (f_equal (fun st => st X)) in H13.
+      apply H13. }
+    rewrite H0 in H1. discriminate.
+Qed.
+(* /ADMITTED -/
+```
+::::
+:::::
+
+:::::full
+The definition of program equivalence we are using here has some
+subtle consequences on programs that may loop forever.  What
+`Equiv` says is that the set of possible _terminating_ outcomes
+of two equivalent programs is the same. However, in a language
+with nondeterminism, like Himp, some programs always terminate,
+some programs always diverge, and some programs can
+nondeterministically terminate in some runs and diverge in
+others. The final part of the following exercise illustrates this
+phenomenon.
+:::::
+
+:::::full
+::::exercise (rating := 4) (name := "p₁_p₂_term") (level := Advanced)
+Consider the following commands:
+
+```lean
+def p₁ : Com :=
+  imp {
+    while (X = 0) {
+       havoc Y;
+       X := X + 1
+    }
+  }
+
+def p₂ : Com :=
+  imp{
+    while (¬ (X = 0)) {
+       skip
+    }
+  }
+
+```
+
+Intuitively, `p₁` and `p₂` have the same termination behavior:
+either they loop forever, or they terminate in the same state they
+started in.  We can capture the termination behavior of `p₁` and
+`p₂` individually with these lemmas:
+
+```lean
+theorem p₁_may_diverge (st st' : State) (h : st[X] ≠ 0) :
+  ¬ (st =[ p₁ ]=> st') := by
+  solution!
+    sorry
+    /- Proof. (* ADMITTED
+      intros. intros Hcontra.
+      remember p₁ as p₁' eqn:Heqp₁'. remember st' as st'' eqn:Heqst''.
+      induction Hcontra; inversion Heqp₁'.
+      - (* E_WhileFalse  subst. simpl in H0.
+        apply negb_false_iff in H0. apply eqb_eq in H0.
+        apply H in H0. assumption.
+      - (* E_WhileTrue  subst. apply IHHcontra2; try reflexivity.
+        inversion Hcontra1. subst.
+        inversion H3; subst. inversion H6; subst.
+        rewrite t_update_eq. simpl. lia.
+    Qed. -/
+```
+
+:::gradeTheorem 3 p₁_may_diverge
+:::
+
+```lean
+theorem p₂_may_diverge (st st' : State) (h : st[X] ≠ 0) :
+  ¬ (st =[ p₂ ]=> st') := by
+  solution!
+    sorry
+/- (* ADMITTED
+  intros. intros Hcontra.
+  remember p₂ as p₂' eqn:Heqp₂'. remember st' as st'' eqn:Heqst''.
+  induction Hcontra; inversion Heqp₂'.
+  - (* E_WhileFalse  subst. simpl in H0.
+    apply negb_false_iff in H0. apply eqb_eq in H0.
+    apply H in H0. assumption.
+  - (* E_WhileTrue  subst. apply IHHcontra2; try reflexivity.
+    inversion Hcontra1. subst.
+    assumption.
+Qed. (* /ADMITTED -/
+```
+
+:::gradeTheorem 3 p₂_may_diverge
+:::
+::::
+:::::
+
+:::::full
+::::exercise (rating := 4) (name := "p₁_p₂_equiv") (level := Advanced)
+Use these two lemmas to prove that `p₁` and `p₂` are actually
+equivalent.
+
+```lean
+theorem p₁_p₂_equiv : p₁ ≃ p₂ := by
+  solution!
+    sorry
+    /- Proof. (* ADMITTED
+      split; intros.
+      - remember p₁ as p₁' eqn:Heqp₁'.
+        destruct H; inversion Heqp₁'; subst.
+        + (* E_WhileFalse  apply E_WhileFalse. assumption.
+        + (* E_WhileTrue  apply p₁_may_diverge in H1.
+          * inversion H1.
+          * simpl in H. apply negb_true_iff in H. apply eqb_neq in H.
+            inversion H0. subst. inversion H4. subst. inversion H7. subst.
+            rewrite t_update_eq. simpl. lia.
+      - remember p₂ as p₂' eqn:Heqp₂'.
+        destruct H; inversion Heqp₂'; subst.
+        + (* E_WhileFalse  apply E_WhileFalse. assumption.
+        + (* E_WhileTrue  apply p₂_may_diverge in H1.
+          * inversion H1.
+          * simpl in H. apply negb_true_iff in H. apply eqb_neq in H.
+            inversion H0. subst. assumption.
+    Qed. (* /ADMITTED -/
+```
+
+:::gradeTheorem 6 p₁_p₂_equiv
+:::
+
+::::
+:::::
+
+:::::full
+::::exercise (rating := 4) (name := "p₃_p₄_inequiv") (level := Advanced)
+Prove that the following programs are _not_ equivalent.  (Hint:
+What should the value of `Z` be when `p₃` terminates?  What about
+`p₄`?)
+
+```lean
+def p₃ : Com :=
+  imp {
+    Z := 1;
+    while (X ≠ 0) {
+      havoc X;
+      havoc Z
+    }
+  }
+
+def p₄ : Com :=
+  imp {
+    X := 0;
+    Z := 1
+  }
+```
+
+:::solution
+First, note that the programs `p₃` and `p₄` are not equivalent:
+when `p₃` terminates, even though `X` definitely has value `0`,
+`Z` might have any natural number as the value.
+:::
+
+```lean
+theorem p₃_p₄_inequiv : ¬ (p₃ ≃ p₄) := by
+  solution!
+    sorry
+   /- Proof. (* ADMITTED
+      intros Hcontra.
+      unfold cequiv in Hcontra.
+      remember (X →ₜ 1) as st.
+      assert (st =[ p₃ ]=> (Z →ₜ 0 ; X →ₜ 0 ; Z →ₜ 1 ; st)).
+      - eapply E_Seq.
+        + constructor. reflexivity.
+        + simpl. eapply E_WhileTrue.
+          * subst. reflexivity.
+          * eapply E_Seq; constructor.
+          * apply E_WhileFalse.
+            reflexivity.
+      - apply Hcontra in H.
+        inversion H. subst.
+        inversion H2. subst.
+        inversion H5. subst.
+        simpl in H6.
+        apply (f_equal (fun st => st Z)) in H6.
+        discriminate H6.
+    Qed. (* /ADMITTED -/
+```
+
+:::gradeTheorem 6 p₃_p₄_inequiv
+:::
+
+::::
+:::::
+
+
+
+:::::full
+::::exercise (rating := 5) (name := "p₅_p₆_equiv") (level := Advanced) (optional := true)
+Prove that the following commands are equivalent.  (Hint: As
+mentioned above, our definition of `Equiv` for Himp only takes
+into account the sets of possible terminating configurations: two
+programs are equivalent if and only if the set of possible terminating
+states is the same for both programs when given a same starting state
+`st`.  If `p₅` terminates, what should the final state be? Conversely,
+is it always possible to make `p₅` terminate?)
+
+```lean
+def p₅ : Com :=
+  imp {
+    while (X ≠ 1) {
+      havoc X
+    }
+  }
+
+def p₆ : Com := imp { X := 1 }
+```
+
+:::solution
+Programs `p₅` and `p₆` are equivalent although `p₅` may diverge,
+while `p₆` always terminates. The definition we took for `Equiv`
+cannot distinguish between these two scenarios. It accepts the two
+programs as equivalent on the basis that: if `p₅` terminates it
+produces the same final state as `p₆`, and there exists an
+execution in which `p₅` terminates and does exactly as `p₆`.
+
+There are two directions to the proof:
+
+`→`: Observe that whenever `p₅` terminates, it does so with `X`
+set to `1`, and no other variable changed. But this is exactly the
+behavior of `p₆`. Thus given a pair of states `st` and `st'` and
+that `st =[ p₅ ]=> st'`, the answer to the question
+"Does `st =[ p₆ ]=> st'`?"  is "Yes".
+
+`←` (and more controversially): Given that `st =[ p₆ ]=> st'` for
+some `st` and `st'`, can we show that `st =[ p₅ ]=> st'`? Observe
+that we can use the hypothesis to conclude that
+`st' = (X →ₜ 1 ; st)`.
+Is there some execution of `p₅` starting from `st` which also
+ends up in `st'`? Yes!
+
+Hence their equivalence.
+
+```lean
+theorem p₅_summary (st st' : State) (h : st =[ p₅ ]=> st') : st' = (X →ₜ 1 ; st) := by sorry
+/- Proof.
+  intros. remember p₅ as p₅' eqn:Heqp₅'.
+  induction H; inversion Heqp₅'; subst.
+  - (* E_WhileFalse
+    simpl in H. apply negb_false_iff in H. apply eqb_eq in H.
+    rewrite <- H. rewrite t_update_same. reflexivity.
+  - (* E_WhileTrue
+    apply IHceval₂ in Heqp₅'.
+    inversion H0; subst.
+    apply t_update_shadow. -/
+```
+:::
+
+```lean
+theorem p₅_p₆_equiv : p₅ ≃ p₆ := by
+  solution!
+    sorry
+    /- Proof. (* ADMITTED
+      split; intros.
+      - (* →
+        apply p₅_summary in H. subst. constructor. reflexivity.
+      - (* <-  inversion H. subst.
+        simpl. simpl in H.
+        destruct ((st X) = 1) eqn:Heqb.
+        + (* X = 1
+          apply eqb_eq in Heqb.
+          rewrite <- Heqb.
+          rewrite t_update_same.
+          apply E_WhileFalse. simpl. rewrite → Heqb.
+          reflexivity.
+        + (* X ≠ 1
+          apply E_WhileTrue with (st' := (X →ₜ 1 ; st)).
+          * simpl. rewrite Heqb. reflexivity.
+          * constructor.
+          * apply E_WhileFalse. reflexivity. -/
+```
+::::
+
+```lean
+end Himp
+```
+:::::
+
+# Additional Exercises
+
+:::suppressPreviousHeaderWhenTerse
+:::
+
+:::::full
+::::exercise (rating := 3) (name := "swap_noninterfering_assignments") (optional := true)
+(Hint: You may or may not - depending how you approach it - need
+to use `ext` explicitly for this one.)
+
+```lean
+theorem swap_noninterfering_assignments (l₁ l₂ : String) (a₁ a₂ : Aexp)
+  (hl : l₁ ≠ l₂)
+  (h₁ : VarNotUsedInAexp l₁ a₂)
+  (h₂ : VarNotUsedInAexp l₂ a₁) :
+  imp { l₁ := a₁; l₂ := a₂ } ≃ imp { l₂ := a₂; l₁ := a₁ } := by
+    solution!
+      sorry
+      /- Proof.
+      (* ADMITTED
+        assert (HS : forall l₁ l₂ a₁ a₂,
+          l₁ ≠ l₂ →
+          VarNotUsedInAexp l₁ a₂ →
+          VarNotUsedInAexp l₂ a₁ →
+          forall st st',
+            st =[ l₁ := a₁; l₂ := a₂ ]=> st' →
+            st =[ l₂ := a₂; l₁ := a₁ ]=> st').
+        { intros l₁ l₂ a₁ a₂ Hneq HNE1 HNE2 st st' H.
+          inversion H; subst. inversion H2; subst. inversion H5; subst.
+          eapply E_Seq.
+          - apply E_Asgn. reflexivity.
+          - rewrite → (t_update_permute _ _ _ _ _ _ Hneq).
+            replace (aeval (l₁ →ₜ a₁; st) a₂) with a₂.eval st..eval st
+            + apply E_Asgn. apply aeval_weakening. apply HNE2.
+            + symmetry. apply aeval_weakening. apply HNE1. }
+        split; eauto.
+      Qed. (* /ADMITTED -/
+```
+::::
+:::::
+
+:::::full
+::::exercise (rating := 4) (name := "for_while_equiv") (optional := true)
+This exercise extends the optional `add_for_loop` exercise from
+the {ref "Imp"}[Imp] chapter, where you were asked to extend the language
+of commands with C-style `for` loops.  Prove that the command:
+
+```
+for (c₁; b; c₂) {
+  c₃
+}
+```
+
+is equivalent to:
+
+```
+c₁;
+while (b) {
+  c₃;
+  c₂
+}
+```
+::::
+:::::
+
+:::::full
+::::exercise (rating := 4) (name := "cApprox") (level := Advanced) (optional := true)
+In this exercise we define an asymmetric variant of program
+equivalence we call _program approximation_. We say that a
+program `c₁` _approximates_ a program `c₂` when, for each of
+the initial states for which `c₁` terminates, `c₂` also terminates
+and produces the same final state. Formally, program approximation
+is defined as follows:
+
+```lean
+def Approx (c₁ c₂ : Com) : Prop := forall (st st' : State),
+  (st =[ c₁ ]=> st') → (st =[ c₂ ]=> st')
+```
+
+For example, the program `c₁`
+
+```
+while (X ≠ 1) {
+  X := X - 1
+}
+```
+
+approximates `c₂`: `X := 1`, but `c₂` does not approximate `c₁`
+since `c₁` does not terminate when `X = 0` but `c₂` does.  If two
+programs approximate each other in both directions, then they are
+equivalent.
+
+Find two programs `c₃` and `c₄` such that neither approximates
+the other.
+
+```lean
+def c₃ : Com :=
+-- SOLUTION
+  imp { X := 1 }
+-- END SOLUTION
+def c₄ : Com :=
+-- SOLUTION
+  imp { X := 2 }
+-- END SOLUTION
+```
+
+```lean
+theorem c₃_c₄_different : ¬ (Approx c₃ c₄) ∧ ¬ (Approx c₄ c₃) := by
+  solution!
+    sorry
+    /- Proof. (* ADMITTED
+      unfold not, capprox; split; intros.
+
+      - assert (empty_st =[ c₃ ]=> (X →ₜ 1)).
+        + constructor. reflexivity.
+        + apply H in H0. inversion H0; subst. simpl in H5.
+          assert ((X →ₜ 2) X = 2).
+          * reflexivity.
+          * assert ((X →ₜ 1) X = 1).
+            -- reflexivity.
+            -- rewrite → H5 in H1. rewrite → H2 in H1. inversion H1.
+
+      - assert (empty_st =[ c₄ ]=> (X →ₜ 2)).
+        + constructor. reflexivity.
+        + apply H in H0. inversion H0; subst. simpl in H5.
+          assert ((X →ₜ 2) X = 2).
+          * reflexivity.
+          * assert ((X →ₜ 1) X = 1).
+            -- reflexivity.
+            -- rewrite → H5 in H2. rewrite → H1 in H2. inversion H2.
+    Qed. (* /ADMITTED-/
+```
+
+Find a program `cMin` that approximates every other program.
+
+```lean
+def cMin : Com :=
+-- SOLUTION
+  imp { while (true) { skip } }
+-- END SOLUTION
+
+theorem cMin_minimal (c : Com) : Approx cMin c := by
+  solution!
+    sorry
+    /- Proof. (* ADMITTED
+      unfold capprox. intros.
+      apply loop_never_stops in H.
+      inversion H.
+    Qed. (* /ADMITTED -/
+```
+
+Finally, find a non-trivial property which is preserved by
+program approximation (when going from left to right).
+
+```lean
+def zprop (c : Com) : Prop :=
+-- SOLUTION
+  forall st, exists st', (st =[ c ]=> st')
+-- END SOLUTION
+```
+
+:::solution
+Intuitively, `zprop` holds of programs that terminate on all
+inputs.
+:::
+
+```lean
+theorem zprop_preserving (c c' : Com) (hc : zprop c) (ha : Approx c c') : zprop c' := by
+  solution!
+    sorry
+      /- Proof. (* ADMITTED
+        unfold zprop, capprox. intros.
+        specialize (H st). inversion H as `st'`.
+        apply H0 in H1. exists st'. assumption.
+      Qed. -/
+```
+::::
+:::::
